compcertox/Encapsulation.v
@@ -1,0 +1,2085 @@
+(** Preliminary experiments about incorporating state encapsulation into
+  CompCert languages *)
+
+From compcert Require Import
+     AST Coqlib Maps Values Integers Errors Events
+     LanguageInterface Smallstep Globalenvs Memory Floats.
+From compcert Require Import
+     CategoricalComp.
+From compcertox Require Import
+     TensorComp Lifting.
+From coqrel Require Import RelClasses.
+
+Set Implicit Arguments.
+Generalizable All Variables.
+
+Typeclasses eauto := 20.
+
+(** * State Encapsulation of CompCert LTS *)
+
+(** ** Preliminaries *)
+Class PSet (T: Type) : Type :=
+  pset_init : T.
+
+Instance pset_unit: PSet unit :=
+  { pset_init := tt }.
+
+Instance pset_prod `{PSet A} `{PSet B} : PSet (A * B) | 8 :=
+  { pset_init := (pset_init, pset_init) }.
+(* Infix "*" := pset_prod. *)
+
+(* embed a regular type into a pointed set *)
+Instance pset_option (T: Type) : PSet (option T) :=
+  { pset_init := None }.
+
+Record ReflTranRel (X: Type) :=
+  {
+    rel :> X -> X -> Prop;
+    rel_refl : Reflexive rel;
+    rel_tran : Transitive rel;
+  }.
+Existing Instance rel_refl.
+Existing Instance rel_tran.
+
+(* A generalized version of Kripke world *)
+Class World (T: Type) :=
+  {
+    w_pset: PSet T;
+    (* internal transition step *)
+    w_int_step : ReflTranRel T;
+    (* external transition step *)
+    w_ext_step : ReflTranRel T;
+  }.
+Arguments w_int_step {_ _}.
+Arguments w_ext_step {_ _}.
+Infix "*->" := w_int_step (at level 60, no associativity).
+Infix ":->" := w_ext_step (at level 60, no associativity).
+Existing Instance w_pset | 10.
+
+Instance world_unit : World unit | 1 :=
+  {
+    w_int_step := {| rel s t := True; |};
+    (* external steps maintain the state *)
+    w_ext_step := {| rel s t := True |};
+  }.
+
+Instance pset_world `{PSet T} : World T | 9 :=
+  {
+    w_int_step := {| rel s t := True; |};
+    (* external steps maintain the state *)
+    w_ext_step := {| rel := eq |};
+  }.
+
+Program Instance world_prod `(World A) `(World B) : World (A * B) | 8 :=
+  {
+    w_int_step := {| rel '(u, v) '(u', v') := u *-> u' /\ v *-> v' |};
+    w_ext_step := {| rel '(u, v) '(u', v') := u :-> u' /\ v :-> v' |};
+  }.
+Next Obligation. intros x. destruct x. split; reflexivity. Qed.
+Next Obligation.
+  intros [a b] [c d] [e f] [? ?] [? ?].
+  split; etransitivity; eauto.
+Qed.
+Next Obligation. intros x. destruct x. split; reflexivity. Qed.
+Next Obligation.
+  intros [a b] [c d] [e f] [? ?] [? ?].
+  split; etransitivity; eauto.
+Qed.
+(* Infix "*" := world_prod: world_scope. *)
+(* Delimit Scope world_scope with world. *)
+(* Bind Scope world_scope with world. *)
+
+(* Generate a world that corresponds to the world in vanilla simulation
+   conventions, where the replies are matched at the same world as in the
+   queries and the environment is free to choose a new world to match queries *)
+Instance world_option (T: Type) : World (option T) :=
+  {|
+    w_int_step := {| rel := OptionRel.option_le (fun _ _ => True) |};
+    w_ext_step := {| rel := OptionRel.option_le eq |};
+  |}.
+
+Instance world_symtbl : World (option Genv.symtbl) :=
+  {|
+    w_int_step := {| rel := eq |};
+    w_ext_step := {| rel := OptionRel.option_le eq |};
+  |}.
+
+(** ** Semantics with Encapsulation *)
+Record esemantics {liA liB} := {
+    pstate : Type;              (** persistent state *)
+    pstate_pset : PSet pstate;
+    esem :> semantics liA (liB @ pstate)
+  }.
+Arguments esemantics : clear implicits.
+Infix "+->" := esemantics (at level 70).
+Existing Instance pstate_pset.
+
+(** *** Composition *)
+
+Definition comp_esem' `(L1: liB +-> liC) `(L2: liA +-> liB) sk : liA +-> liC :=
+  {|
+    pstate := pstate L1 * pstate L2;
+    esem := $(comp_semantics' (L1 @ pstate L2) L2 sk);
+  |}.
+
+Definition comp_esem `(L1: liB +-> liC) `(L2: liA +-> liB) : option (liA +-> liC) :=
+  match comp_semantics $(L1 @ pstate L2) L2 with
+  | Some L => Some {| pstate := pstate L1 * pstate L2; esem := L; |}
+  | None => None
+  end.
+
+(** *** Construction *)
+
+Definition semantics_fbk `{PSet K} {liA liB} (L: liA +-> liB@K) : liA +-> liB :=
+  {|
+    pstate := K * pstate L; esem := $L
+  |}.
+
+Definition semantics_embed `(L: semantics liA liB) : liA +-> liB :=
+  {|
+    pstate := unit; esem := semantics_map L lf (li_iso_inv _);
+  |}.
+
+(** ** Stateful Simulation Convention and Simulation *)
+Require Import Relation_Operators.
+
+Module ST.
+
+  Record callconv  {li1 li2} :=
+    mk_callconv {
+      ccworld : Type;
+      ccworld_world : World ccworld;
+      (* match_senv : ccworld -> Genv.symtbl -> Genv.symtbl -> Type; *)
+      match_query : ccworld -> query li1 -> query li2 -> Prop;
+      match_reply : ccworld -> reply li1 -> reply li2 -> Prop;
+    }.
+  Arguments callconv: clear implicits.
+  Existing Instance ccworld_world | 3.
+
+  Program Definition callconv_lift
+          `(cc: callconv li1 li2) `{PSet U} `{PSet V} : callconv (li1@U) (li2@V) :=
+    {|
+      ccworld := ccworld cc * U * V;
+      (* match_senv '(w, u, v) se1 se2 := match_senv cc w se1 se2; *)
+      match_query '(w, u, v) '(q1, uq) '(q2, vq) :=
+        match_query cc w q1 q2 /\ u = uq /\ v = vq;
+      match_reply '(w, u, v) '(q1, uq) '(q2, vq) :=
+        match_reply cc w q1 q2 /\ u = uq /\ v = vq;
+    |}.
+
+  Program Definition cc_compose {li1 li2 li3}
+          (cc12: callconv li1 li2) (cc23: callconv li2 li3) :=
+    {|
+      ccworld := ccworld cc12 * ccworld cc23;
+      (* match_senv '(w12, w23) se1 se3 := *)
+      (*   { se2 & (match_senv cc12 w12 se1 se2 * match_senv cc23 w23 se2 se3)%type }; *)
+      match_query '(w12, w23) q1 q3 :=
+      exists q2,
+        match_query cc12 w12 q1 q2 /\
+        match_query cc23 w23 q2 q3;
+      match_reply '(w12, w23) r1 r3 :=
+      exists r2,
+        match_reply cc12 w12 r1 r2 /\
+        match_reply cc23 w23 r2 r3;
+    |}.
+
+  (** Stateful Simulation *)
+  Section FSIM.
+
+    Context {liA1 liA2} (ccA: callconv liA1 liA2).
+    Context {liB1 liB2} (ccB: callconv liB1 liB2).
+    Context (wA: ccworld ccA) (wB: ccworld ccB)
+            (winv: ccworld ccA -> ccworld ccB -> Prop).
+    Context {state1 state2: Type}.
+
+    (* There is supposed to be a relation between the wB and wA, which is
+       re-established at the end *)
+    Record fsim_properties
+           (L1: lts liA1 liB1 state1) (L2: lts liA2 liB2 state2)
+           (index: Type) (order: index -> index -> Prop)
+           (match_states: ccworld ccA -> ccworld ccB -> index -> state1 -> state2 -> Prop) :=
+      {
+        fsim_match_initial_states:
+          forall q1 q2 s1 wB', wB :-> wB' -> match_query ccB wB' q1 q2 -> initial_state L1 q1 s1 ->
+          exists i, exists s2, initial_state L2 q2 s2 /\
+          exists wA' wB'', wA :-> wA' /\ wB' *-> wB'' /\ match_states wA' wB'' i s1 s2;
+        fsim_match_final_states:
+          forall wA wB i s1 s2 r1, match_states wA wB i s1 s2 -> final_state L1 s1 r1 ->
+          exists r2, final_state L2 s2 r2 /\
+          exists wB', wB *-> wB' /\ match_reply ccB wB' r1 r2 /\ winv wA wB';
+        fsim_match_external:
+          forall wA wB i s1 s2 q1, match_states wA wB i s1 s2 -> at_external L1 s1 q1 ->
+          exists q2, at_external L2 s2 q2 /\ exists wA', wA :-> wA' /\ match_query ccA wA' q1 q2 /\
+          forall r1 r2 s1' wA'', wA' *-> wA'' -> match_reply ccA wA'' r1 r2 -> after_external L1 s1 r1 s1' ->
+          exists i' s2', after_external L2 s2 r2 s2' /\
+          exists wA''' wB', wA'' :-> wA''' /\ wB *-> wB' /\ match_states wA''' wB' i' s1' s2';
+        fsim_simulation:
+          forall s1 t s1', Step L1 s1 t s1' ->
+          forall wA wB i s2, match_states wA wB i s1 s2 ->
+          exists i', exists s2', (Plus L2 s2 t s2' \/ (Star L2 s2 t s2' /\ order i' i)) /\
+          exists wA' wB', wA :-> wA' /\ wB *-> wB' /\ match_states wA' wB' i' s1' s2';
+      }.
+    Arguments fsim_properties : clear implicits.
+
+    Lemma fsim_simulation':
+      forall L1 L2 index order match_states, fsim_properties L1 L2 index order match_states ->
+      forall i s1 t s1', Step L1 s1 t s1' ->
+      forall wA wB s2, match_states wA wB i s1 s2 ->
+      exists i' wA' wB', wA :-> wA' /\ wB *-> wB' /\
+      ((exists s2', Plus L2 s2 t s2' /\ match_states wA' wB' i' s1' s2')
+      \/ (order i' i /\ t = E0 /\ match_states wA' wB' i' s1' s2)).
+    Proof.
+      intros. exploit @fsim_simulation; eauto.
+      intros (i' & s2' & A & wai & wbi & Hai & Hbi & B).
+      exists i', wai, wbi. repeat split; eauto.
+      destruct A.
+      left; exists s2'; auto.
+      destruct H2. inv H2.
+      right; eauto.
+      left; exists s2'; split; auto. econstructor; eauto.
+    Qed.
+
+    Section SIMULATION_SEQUENCES.
+
+      Context L1 L2 index order match_states
+              (S: fsim_properties L1 L2 index order match_states).
+
+      Lemma simulation_star:
+        forall s1 t s1', Star L1 s1 t s1' ->
+        forall wA wB i s2, match_states wA wB i s1 s2 ->
+        exists wA' wB' i', exists s2', Star L2 s2 t s2' /\
+        wA :-> wA' /\ wB *-> wB' /\ match_states wA' wB' i' s1' s2'.
+      Proof.
+        induction 1; intros.
+        eexists _, _, i; exists s2; repeat split; auto. apply star_refl.
+        reflexivity. reflexivity. assumption.
+        exploit fsim_simulation; eauto.
+        intros (i' & s2' & A & wai & wbi & Hai & Hbi & B).
+        exploit IHstar; eauto.
+        intros (waj & wbj & i'' & s2'' & Hx & Haj & Hbj & C).
+        exists waj, wbj, i''; exists s2''; repeat split; auto.
+        eapply star_trans; eauto.
+        intuition auto. apply plus_star; auto.
+        all: etransitivity; eauto.
+      Qed.
+
+      Lemma simulation_plus:
+        forall s1 t s1', Plus L1 s1 t s1' ->
+        forall wA wB i s2, match_states wA wB i s1 s2 ->
+        exists wA' wB' i', wA :-> wA' /\ wB *-> wB' /\
+        ((exists s2', Plus L2 s2 t s2' /\ match_states wA' wB' i' s1' s2') \/
+        clos_trans _ order i' i /\ t = E0 /\ match_states wA' wB' i' s1' s2).
+      Proof.
+        induction 1 using plus_ind2; intros.
+        (* base case *)
+        - exploit fsim_simulation'; eauto.
+          intros (i' & wai & wbi & Hai & Hbi & A).
+          exists wai, wbi, i'. repeat split; eauto.
+          destruct A.
+          left; auto.
+          right; intuition.
+        (* inductive case *)
+        - exploit fsim_simulation'; eauto.
+          intros (i' & wai & wbi & Hai & Hbi & A).
+          destruct A as [[s2' [A B]] | [A [B C]]].
+          + exploit simulation_star. apply plus_star; eauto. eauto.
+            intros (waj & wbj & i'' & s2'' & P & Haj & Hbj & Q).
+            exists waj, wbj, i''. repeat split. 1-2: etransitivity; eauto.
+            left; exists s2''; split; auto. eapply plus_star_trans; eauto.
+
+          + exploit IHplus; eauto.
+            intros (waj & wbj & i'' & Haj & Hbj & P).
+            destruct P as [[s2'' [P Q]] | [P [Q R]]].
+            * subst. simpl.
+              exists waj, wbj, i''. repeat split. 1-2: etransitivity; eauto.
+              left; exists s2''; auto.
+            * subst. simpl.
+              exists waj, wbj, i''. repeat split. 1-2: etransitivity; eauto.
+              right; intuition auto.
+              eapply t_trans; eauto. eapply t_step; eauto.
+      Qed.
+
+    End SIMULATION_SEQUENCES.
+  End FSIM.
+
+  Arguments fsim_properties {_ _} _ {_ _} _ _ _ _ {_ _} L1 L2 index order match_states.
+
+  Record fsim_components {liA1 liA2} (ccA: callconv liA1 liA2)
+         {liB1 liB2} (ccB: callconv liB1 liB2) L1 L2 :=
+    Forward_simulation {
+        fsim_index: Type;
+        fsim_order: fsim_index -> fsim_index -> Prop;
+        fsim_match_states: _;
+        fsim_invariant: ccworld ccA -> ccworld ccB -> Prop;
+
+        fsim_invariant_env_step:
+          forall wA wB, fsim_invariant wA wB -> forall wB', wB :-> wB' -> fsim_invariant wA wB';
+        fsim_skel: skel L1 = skel L2;
+        fsim_initial_world: fsim_invariant (@pset_init (ccworld ccA) _)
+                                           (@pset_init (ccworld ccB) _);
+        fsim_footprint: forall i, footprint L1 i <-> footprint L2 i;
+        fsim_lts wA wB se:
+          fsim_invariant wA wB ->
+          fsim_properties ccA ccB wA wB fsim_invariant (activate L1 se) (activate L2 se)
+                          fsim_index fsim_order (fsim_match_states se);
+        fsim_order_wf:
+          well_founded fsim_order;
+      }.
+  Arguments Forward_simulation {_ _ ccA _ _ ccB L1 L2 fsim_index}.
+
+  Definition forward_simulation {liA1 liA2} ccA {liB1 liB2} ccB L1 L2 :=
+    inhabited (@fsim_components liA1 liA2 ccA liB1 liB2 ccB L1 L2).
+
+End ST.
+Arguments ST.callconv_lift {_ _} _ _ {_} _ {_}.
+
+(** Normalized Stateful Simulation *)
+Module STCAT.
+  Definition forward_simulation {liA1 liA2} (ccA: ST.callconv liA1 liA2)
+             {liB1 liB2} (ccB: ST.callconv liB1 liB2) L1 L2 :=
+    ST.forward_simulation ccA ccB (normalize_sem L1) (normalize_sem L2).
+End STCAT.
+
+(** Simulations between components with encapsulated states *)
+Module E.
+  Definition forward_simulation {liA1 liA2} (ccA: ST.callconv liA1 liA2)
+             {liB1 liB2} (ccB: ST.callconv liB1 liB2)
+             (L1: liA1 +-> liB1) (L2: liA2 +-> liB2) :=
+    STCAT.forward_simulation ccA (ST.callconv_lift ccB (pstate L1) (pstate L2)) L1 L2.
+End E.
+
+(** * Properties about Stateful Simulations *)
+
+(** ** Embedding Stateless Simulations *)
+
+Definition callconv_embed {liA liB} (cc: callconv liA liB)
+           `{World (ccworld cc)}: ST.callconv liA liB :=
+  {|
+    ST.ccworld := ccworld cc;
+    ST.match_query := match_query cc;
+    ST.match_reply := match_reply cc;
+  |}.
+Notation "& cc" := (callconv_embed cc) (at level 0).
+
+Hypothesis fsim_embed:
+  forall `(ccA: callconv liA1 liA2) `{!World (ccworld ccA)}
+    `(ccB: callconv liB1 liB2) `{World (ccworld ccB)} L1 L2,
+    forward_simulation ccA ccB L1 L2 -> ST.forward_simulation &ccA &ccB L1 L2.
+
+(** ** Lifting Simulations with Additional States *)
+
+Section LIFT.
+
+  Context `(ccA: ST.callconv liA1 liA2)
+          `(ccB: ST.callconv liB1 liB2)
+          `(X: ST.fsim_components ccA ccB L1 L2).
+  Context `{PSet K1} `{PSet K2}.
+
+  Lemma st_fsim_lift': ST.forward_simulation
+                        (ST.callconv_lift ccA K1 K2)
+                        (ST.callconv_lift ccB K1 K2)
+                        (L1@K1) (L2@K2).
+  Proof.
+    constructor.
+    eapply ST.Forward_simulation with
+      (ST.fsim_order X)
+      (fun se '(wa, k1a, k2a) '(wb, k1b, k2b) i '(s1, k1) '(s2, k2) =>
+         ST.fsim_match_states X se wa wb i s1 s2 /\
+           k1a = k1 /\ k1b = k1 /\ k2a = k2 /\ k2b = k2)
+      (fun '(wa, k1a, k2a) '(wb, k1b, k2b) => ST.fsim_invariant X wa wb /\ k1a = k1b /\ k2a = k2b).
+    - intros [[wa k1a] k2a] [[wb k1b] k2b] (INV & -> & ->) [[wb' k1b'] k2b'] W.
+      destruct W as [[W U] V]. inv U. inv V. repeat split; eauto.
+      eapply ST.fsim_invariant_env_step; eauto.
+    - apply X.
+    - cbn. repeat split; eauto. apply X.
+    - intros i. cbn. apply X.
+    - intros [[wa k1a] k2a] [[wb k1b] k2b] se (I & -> & ->). split; cbn.
+      + intros. eprod_crush. subst.
+        pose proof (ST.fsim_lts X _ _ se I).
+        edestruct @ST.fsim_match_initial_states as (idx & s' & Hs' & Hs); eauto.
+        destruct Hs as (wa' & wb'' & W1 & W2 & HS).
+        eexists idx, (s', _). repeat split; eauto.
+        eexists (wa', _, _), (wb'', _, _). repeat split; eauto.
+      + intros. eprod_crush. subst.
+        pose proof (ST.fsim_lts X _ _ se I).
+        edestruct @ST.fsim_match_final_states as (r' & H' & Hr'); eauto.
+        destruct Hr' as (wb' & W & Hr' & INV).
+        eexists (r', _). repeat split; eauto.
+        eexists (wb', _, _). repeat split; eauto.
+      + intros. eprod_crush. subst.
+        pose proof (ST.fsim_lts X _ _ se I).
+        edestruct @ST.fsim_match_external as (q' & H' & wa' & WA & Hq' & HH); eauto.
+        eexists (q', _). repeat split; eauto.
+        eexists (wa', _, _). repeat split; eauto.
+        intros. eprod_crush. subst.
+        edestruct HH as (i' & s2' & Haft & Hs); eauto.
+        destruct Hs as (wa'' & wb' & WA' & WB & HS).
+        eexists i', (s2', _). repeat split; eauto.
+        eexists (wa'', _, _), (wb', _, _). repeat split; eauto.
+      + intros. eprod_crush. subst.
+        pose proof (ST.fsim_lts X _ _ se I).
+        edestruct @ST.fsim_simulation as (idx' & s2' & Hs2' & Hs'); eauto.
+        destruct Hs' as (wa' & wb' & WA & WB & HS).
+        destruct Hs2'.
+        * eexists idx', (s2', _). split.
+          -- left. apply lifting_step_plus; eauto.
+          -- eexists (wa', _, _), (wb', _, _).
+             repeat split; eauto.
+        * eexists idx', (s2', _). split.
+          -- right. split. apply lifting_step_star; eauto. all: apply H4.
+          -- eexists (wa', _, _), (wb', _, _).
+             repeat split; eauto.
+    - apply X.
+  Qed.
+
+End LIFT.
+
+Lemma st_fsim_lift `(ccA: ST.callconv liA1 liA2) `(ccB: ST.callconv liB1 liB2)
+      L1 L2 `{PSet K1} `{PSet K2}:
+  ST.forward_simulation ccA ccB L1 L2 ->
+  ST.forward_simulation (ST.callconv_lift ccA K1 K2)
+                        (ST.callconv_lift ccB K1 K2)
+                        (L1@K1) (L2@K2).
+Proof. intros [X]. apply st_fsim_lift'. apply X. Qed.
+
+(** ** Composition of Stateful Simulations *)
+
+Section FSIM.
+  Context `(ccA: ST.callconv liA1 liA2)
+          `(ccB: ST.callconv liB1 liB2)
+          `(ccC: ST.callconv liC1 liC2)
+          (L1s: semantics liB1 liC1) (L2s: semantics liA1 liB1)
+          (L1t: semantics liB2 liC2) (L2t: semantics liA2 liB2).
+  Context (HL1: ST.fsim_components ccB ccC L1s L1t)
+          (HL2: ST.fsim_components ccA ccB L2s L2t)
+          (wA : ST.ccworld ccA) (wC: ST.ccworld ccC)
+          (se: Genv.symtbl).
+
+  Variant index := | index1: ST.fsim_index HL1 -> index
+                   | index2: ST.fsim_index HL1 -> ST.fsim_index HL2 -> index.
+
+  Variant order: index -> index -> Prop :=
+    | order1 i1 i1': ST.fsim_order HL1 i1 i1' ->
+                     order (index1 i1) (index1 i1')
+    | order2 i1 i2 i2': ST.fsim_order HL2 i2 i2' ->
+                        order (index2 i1 i2) (index2 i1 i2').
+
+  Inductive match_states: ST.ccworld ccA -> ST.ccworld ccC -> index ->
+                          comp_state L1s L2s -> comp_state L1t L2t -> Prop :=
+  | match_st1 wa wb wc i1 s1 s1':
+    ST.fsim_match_states HL1 se wb wc i1 s1 s1' ->
+    ST.fsim_invariant HL2 wa wb ->
+    match_states wa wc (index1 i1) (st1 L1s L2s s1) (st1 L1t L2t s1')
+  | match_st2 wa wb wc i1 i2 s1 t1 s2 t2 :
+    ST.fsim_match_states HL2 se wa wb i2 s2 t2 ->
+    (forall r1 r2 (s1' : state L1s) wb',
+        wb *-> wb' ->
+        ST.match_reply ccB wb' r1 r2 ->
+        after_external (L1s se) s1 r1 s1' ->
+        exists (i' : ST.fsim_index HL1) (t1' : state L1t),
+          after_external (L1t se) t1 r2 t1' /\
+            exists wb'' wc', wb' :-> wb'' /\ wc *-> wc' /\
+            ST.fsim_match_states HL1 se wb'' wc' i' s1' t1') ->
+    match_states wa wc (index2 i1 i2) (st2 L1s L2s s1 s2) (st2 L1t L2t t1 t2).
+
+  Definition inv : ST.ccworld ccA -> ST.ccworld ccC -> Prop :=
+    fun wa wc => exists wb, ST.fsim_invariant HL1 wb wc /\ ST.fsim_invariant HL2 wa wb.
+
+  Lemma st_fsim_lcomp' sk sk':
+    inv wA wC ->
+    ST.fsim_properties ccA ccC wA wC inv
+                       (comp_semantics' L1s L2s sk se)
+                       (comp_semantics' L1t L2t sk' se)
+                       index order match_states.
+  Proof.
+    intros (wB & INV1 & INV2). split; cbn.
+    - intros q1 q2 s1 wC' WC Hq H. inv H.
+      pose proof (ST.fsim_lts HL1 _ _ se INV1).
+      edestruct @ST.fsim_match_initial_states as (idx & s' & Hs' & Hs); eauto.
+      destruct Hs as (wB' & wC'' & W1 & W2 & HS).
+      exists (index1 idx), (st1 L1t L2t s').
+      split. econstructor; eauto.
+      exists wA, wC''. repeat split; eauto. reflexivity.
+      econstructor. apply HS. eapply ST.fsim_invariant_env_step; eauto.
+    - intros wa wb i s1 s2 r1 Hs Hf. inv Hf. inv Hs.
+      rename wb into wc. rename wb0 into wb.
+      pose proof (ST.fsim_lts HL1 _ _ se INV1).
+      edestruct @ST.fsim_match_final_states as (r' & H' & Hr'); eauto.
+      destruct Hr' as (wc' & W & Hr' & INV).
+      exists r'. split. econstructor; eauto.
+      exists wc'. repeat split; eauto.
+      exists wb. split; eauto.
+    - intros wa wc i s1 s2 q1 Hs H. inv H. inv Hs.
+      pose proof (ST.fsim_lts HL2 _ _ se INV2).
+      edestruct @ST.fsim_match_external as (q' & H' & wa' & WA & Hq' & HH); eauto.
+      exists q'. split. econstructor; eauto.
+      exists wa'. repeat split; eauto.
+      intros r1 r2 xs1 wa'' WA' Hr HH'. inv HH'.
+      specialize (HH _ _ _ _ WA' Hr H6) as (i2' & xs2 & Haft & Hss).
+      destruct Hss as (wa''' & wb' & WA'' & WB & HS).
+      eexists (index2 i1 i2'), (st2 L1t L2t _ _).
+      split. econstructor; eauto.
+      exists wa''', wc. repeat split; eauto. reflexivity.
+      econstructor. exact HS.
+      intros ? ? ? wbx WBX. apply H7. etransitivity; eauto.
+    - intros s1 t s2 Hstep wa wc idx t1 Hs.
+      inv Hstep; inv Hs.
+      + pose proof (ST.fsim_lts HL1 _ _ se INV1).
+        edestruct @ST.fsim_simulation as (idx' & s2' & Hs2' & Hs'); eauto.
+        destruct Hs' as (wb' & wc' & WB & WC & HS).
+        exists (index1 idx'), (st1 L1t L2t s2'). split.
+        * destruct Hs2'; [ left | right ].
+          apply plus_internal1. auto.
+          split. apply star_internal1. apply H2. constructor; apply H2.
+        * exists wa, wc'. repeat split; eauto. reflexivity.
+          econstructor; eauto. eapply @ST.fsim_invariant_env_step; eauto.
+      + pose proof (ST.fsim_lts HL2 _ _ se INV2).
+        edestruct @ST.fsim_simulation as (idx' & xs2' & Hs2' & Hs'); eauto.
+        destruct Hs' as (wa' & wb' & WA & WB & HS).
+        exists (index2 i1 idx'), (st2 L1t L2t t0 xs2'). split.
+        * destruct Hs2'; [ left | right ].
+          -- apply plus_internal2. auto.
+          -- split. apply star_internal2. apply H1.
+             constructor. apply H1.
+        * exists wa', wc. repeat split; eauto. reflexivity.
+          econstructor; eauto.
+          intros r1 r2 sr wb'' WB'. apply H7. etransitivity; eauto.
+      + pose proof (ST.fsim_lts HL1 _ _ se INV1).
+        edestruct @ST.fsim_match_external as (q' & H' & wb' & WB & Hq' & HH); eauto.
+        pose proof (ST.fsim_lts HL2 _ _ se H6).
+        edestruct @ST.fsim_match_initial_states as (i2 & s' & Hs' & Hs); eauto.
+        destruct Hs as (wa' & wb'' & WA & WB' & Hs).
+        exists (index2 i1 i2), (st2 L1t L2t s1' s'). split.
+        * left. apply plus_one. eapply step_push; eauto.
+        * exists wa', wc. repeat split; eauto. reflexivity.
+          econstructor; eauto.
+          intros r1 r2 sr wb''' WB'' HR Haft.
+          specialize (HH r1 r2 sr wb'''). apply HH. etransitivity; eauto.
+          exact HR. exact Haft.
+      + pose proof (ST.fsim_lts HL2 _ _ se INV2).
+        edestruct @ST.fsim_match_final_states as (r' & H' & Hr'); eauto.
+        edestruct Hr' as (wb' & WB & Hr & INV).
+        edestruct H8 as (idx & t1 & HH & HX); eauto.
+        destruct HX as (wb'' & wc' & WB' & WC & HS).
+        exists (index1 idx), (st1 L1t L2t t1). split.
+        * left. apply plus_one. eapply step_pop; eauto.
+        * exists wa, wc'. repeat split; eauto. reflexivity.
+          econstructor. exact HS.
+          eapply ST.fsim_invariant_env_step; eauto.
+  Qed.
+
+End FSIM.
+
+Section COMP.
+
+  Context `(ccA: ST.callconv liA1 liA2)
+          `(ccB: ST.callconv liB1 liB2)
+          `(ccC: ST.callconv liC1 liC2)
+          (L1s: semantics liB1 liC1) (L2s: semantics liA1 liB1)
+          (L1t: semantics liB2 liC2) (L2t: semantics liA2 liB2).
+  Context (HL1: ST.forward_simulation ccB ccC L1s L1t)
+          (HL2: ST.forward_simulation ccA ccB L2s L2t).
+  Context `(HLs: comp_semantics L1s L2s = Some Ls)
+          Lt (HLt: comp_semantics L1t L2t = Some Lt).
+
+  Lemma st_fsim_lcomp : ST.forward_simulation ccA ccC Ls Lt.
+  Proof.
+    destruct HL1 as [Ha]. destruct HL2 as [Hb].
+    unfold comp_semantics, option_map in HLs, HLt.
+    destruct (Linking.link (skel L1s) (skel L2s)) as [sk1|] eqn:Hsk1; try discriminate. inv HLs.
+    destruct (Linking.link (skel L1t) (skel L2t)) as [sk2|] eqn:Hsk2; try discriminate. inv HLt.
+    constructor.
+    eapply ST.Forward_simulation
+      with (@order _ _ ccA _ _ ccB _ _ ccC L1s L2s L1t L2t Ha Hb)
+           (@match_states _ _ ccA _ _ ccB _ _ ccC L1s L2s L1t L2t Ha Hb)
+           (@inv _ _ ccA _ _ ccB _ _ ccC L1s L2s L1t L2t Ha Hb).
+    - intros wa wc (wb & I1 & I2) wc' WC.
+      exists wb; split; eauto. eapply ST.fsim_invariant_env_step; eauto.
+    - destruct Ha. destruct Hb. cbn. congruence.
+    - exists (@pset_init (ST.ccworld ccB) _).
+      split. apply Ha. apply Hb.
+    - cbn. intros i. destruct Ha, Hb.
+      rewrite fsim_footprint, fsim_footprint0. reflexivity.
+    - intros wa wc se INV. eapply st_fsim_lcomp'; eauto.
+    - clear - Ha Hb. intros [|].
+      + induction (ST.fsim_order_wf Ha f). constructor.
+        intros. inv H1. apply H0. auto.
+      + induction (ST.fsim_order_wf Hb f0). constructor.
+        intros. inv H1. apply H0. auto.
+  Qed.
+
+  (* TODO: clean up the copy-paste *)
+  Lemma st_fsim_lcomp_sk sk:
+    Linking.linkorder (skel L1s) sk ->
+    Linking.linkorder (skel L2s) sk ->
+    ST.forward_simulation ccA ccC (comp_semantics' L1s L2s sk) (comp_semantics' L1t L2t sk).
+  Proof.
+    intros H1 H2.
+    destruct HL1 as [Ha]. destruct HL2 as [Hb].
+    constructor.
+    eapply ST.Forward_simulation
+      with (@order _ _ ccA _ _ ccB _ _ ccC L1s L2s L1t L2t Ha Hb)
+           (@match_states _ _ ccA _ _ ccB _ _ ccC L1s L2s L1t L2t Ha Hb)
+           (@inv _ _ ccA _ _ ccB _ _ ccC L1s L2s L1t L2t Ha Hb).
+    - intros wa wc (wb & I1 & I2) wc' WC.
+      exists wb; split; eauto. eapply ST.fsim_invariant_env_step; eauto.
+    - destruct Ha. destruct Hb. cbn. congruence.
+    - exists (@pset_init (ST.ccworld ccB) _).
+      split. apply Ha. apply Hb.
+    - cbn. intros i. destruct Ha, Hb.
+      rewrite fsim_footprint, fsim_footprint0. reflexivity.
+    - intros wa wc se INV. eapply st_fsim_lcomp'; eauto.
+    - clear - Ha Hb. intros [|].
+      + induction (ST.fsim_order_wf Ha f). constructor.
+        intros. inv H1. apply H0. auto.
+      + induction (ST.fsim_order_wf Hb f0). constructor.
+        intros. inv H1. apply H0. auto.
+  Qed.
+End COMP.
+
+(** ** Composition of Stateful Simulation Conventions *)
+
+Section COMP_FSIM.
+
+  Context `(ccA1: ST.callconv liAs liAn) `(ccA2: ST.callconv liAn liAf)
+          `(ccB1: ST.callconv liBs liBn) `(ccB2: ST.callconv liBn liBf)
+          (Ls: semantics liAs liBs) (Ln: semantics liAn liBn) (Lf: semantics liAf liBf).
+  Context (H1: ST.fsim_components ccA1 ccB1 Ls Ln)
+          (H2: ST.fsim_components ccA2 ccB2 Ln Lf).
+
+  Inductive compose_fsim_match_states: Genv.symtbl ->
+    ST.ccworld (ST.cc_compose ccA1 ccA2) ->
+    ST.ccworld (ST.cc_compose ccB1 ccB2) ->
+    (ST.fsim_index H2 * ST.fsim_index H1) ->
+    state Ls -> state Lf -> Prop :=
+  | compose_match_states_intro se s1 s2 s3 i1 i2 wa1 wa2 wb1 wb2:
+    ST.fsim_match_states H1 se wa1 wb1 i1 s1 s2 ->
+    ST.fsim_match_states H2 se wa2 wb2 i2 s2 s3 ->
+    compose_fsim_match_states se (wa1, wa2) (wb1, wb2) (i2, i1) s1 s3.
+
+  Inductive compose_fsim_inv:
+    ST.ccworld (ST.cc_compose ccA1 ccA2) ->
+    ST.ccworld (ST.cc_compose ccB1 ccB2) -> Prop :=
+  | compose_fsim_inv_intro wa1 wa2 wb1 wb2:
+    ST.fsim_invariant H1 wa1 wb1 -> ST.fsim_invariant H2 wa2 wb2 ->
+    compose_fsim_inv (wa1, wa2) (wb1, wb2).
+
+  Lemma st_fsim_vcomp':
+    ST.fsim_components (ST.cc_compose ccA1 ccA2)
+                       (ST.cc_compose ccB1 ccB2)
+                       Ls Lf.
+  Proof.
+    (* destruct H1 as [ index1 order1 match_states1 inv1 A1 B1 C1 D1 E1 F1 ]. *)
+    (* destruct H2 as [ index2 order2 match_states2 inv2 A2 B2 C2 D2 E2 F2 ]. *)
+    (* set (ff_index := (index2 * index1)%type). *)
+    set (ff_order := lex_ord (Relation_Operators.clos_trans
+                                _ (ST.fsim_order H2)) (ST.fsim_order H1)).
+    (* set (ff_match_states := *)
+    (*        fun se1 se3 '(ose, wa1, wa2) '(o, wb1, wb2) '(i2, i1) s1 s3 => *)
+    (*          match ose with *)
+    (*          | Some se2 => *)
+    (*              exists s2, match_states1 se1 se2 wa1 wb1 i1 s1 s2 /\ *)
+    (*                      match_states2 se2 se3 wa2 wb2 i2 s2 s3 *)
+    (*          | None => False *)
+    (*          end). *)
+
+    (* set (ff_inv := fun '(x, wa1, wa2) '(y, wb1, wb2) => inv1 wa1 wb1 /\ inv2 wa2 wb2). *)
+
+    (* replace (ST.fsim_index H2 * ST.fsim_index H1)%type *)
+    (*   with ff_index in ff_match_states. *)
+    (* 2: { subst ff_index. rewrite X1. rewrite X2. reflexivity. } *)
+    (* clear X1 X2. *)
+    apply ST.Forward_simulation with ff_order compose_fsim_match_states compose_fsim_inv.
+    - intros [wa1 wa2] [wb1 wb2] I [wb1' wb2'] [X1 X2].
+      inv I. econstructor.
+      eapply (ST.fsim_invariant_env_step H1); eauto.
+      eapply (ST.fsim_invariant_env_step H2); eauto.
+    - rewrite (ST.fsim_skel H1); apply (ST.fsim_skel H2).
+    - econstructor. apply (ST.fsim_initial_world H1).
+      apply (ST.fsim_initial_world).
+    - intros i. rewrite (ST.fsim_footprint H1). apply (ST.fsim_footprint H2).
+    - intros [wa1 wa2] [wb1 wb2] se I. inv I.
+      pose proof (ST.fsim_lts H1 wa1 wb1 se H4) as X1.
+      pose proof (ST.fsim_lts H2 wa2 wb2 se H6) as X2.
+      constructor.
+      + intros q1 q3 s1 (wb1' & wb2') (WB1 & WB2) (q2 & Hq12 & Hq23) Hi.
+        edestruct (@ST.fsim_match_initial_states liAs) as (i & s2 & A & B); eauto.
+        edestruct (@ST.fsim_match_initial_states liAn) as (i' & s3 & C & D); eauto.
+        destruct B as (wa1' & wb1'' & WA1 & WB1' & B).
+        destruct D as (wa2' & wb2'' & WA2 & WB2' & D).
+        eexists (i', i), s3. split; eauto.
+        eexists (wa1', wa2'), (wb1'', wb2''). repeat split; eauto.
+        econstructor; eauto.
+      + intros (wa1' & wa2') (wb1' & wb2') (i2, i1) s1 s3 r1 Hs H.
+        inv Hs.
+        edestruct (@ST.fsim_match_final_states liAs) as (r2 & Hr2 & A); eauto.
+        edestruct (@ST.fsim_match_final_states liAn) as (r3 & Hr3 & B); eauto.
+        destruct A as (wb1'' & WB1' & R1 & I1).
+        destruct B as (wb2'' & WB2' & R2 & I2).
+        exists r3. repeat split; eauto.
+        exists (wb1'', wb2''). repeat split; eauto.
+        econstructor; eauto.
+      + intros (wa1' & wa2') (wb1' & wb2') (i2, i1) s1 s3 q1 Hs H.
+        inv Hs.
+        edestruct (@ST.fsim_match_external liAs) as (q2 & Hq2 & wax & Hwx & Hq12 & Hk12); eauto.
+        edestruct (@ST.fsim_match_external liAn) as (q3 & Hq3 & way & Hwy & Hq23 & Hk23); eauto.
+        exists q3. repeat split; eauto. exists (wax, way). repeat split; eauto.
+        econstructor; eauto.
+        intros r1 r3 s1' (wai, waj) (Hwi & Hwj) (r2 & Hr12 & Hr23) HH.
+        edestruct Hk12 as (i2' & s2' & Hs2' & wam & wbm & Ham & Hbm & Hm); eauto.
+        edestruct Hk23 as (i1' & s3' & Hs3' & wan & wbn & Han & Hbn & Hn); eauto.
+        eexists (_, _), _. repeat split; eauto.
+        eexists (_, _), (_, _). repeat split; eauto.
+        econstructor; eauto.
+      + intros s1 t s1' Hstep (wai & waj) (wbi & wbj) (i2, i1) s3 Hs.
+        inv Hs.
+        edestruct (@ST.fsim_simulation' liAs) as (i1' & waii & wbii & Hai & Hbi & Hx); eauto.
+        destruct Hx as [[s2' [A B]] | [A [B C]]].
+        * (* L2 makes one or several steps. *)
+          edestruct (@ST.simulation_plus liAn) as (wak & wbk & i2' & Hak & Hbk & X); eauto.
+          destruct X as [[s3' [P Q]] | [P [Q R]]].
+          -- (* L3 makes one or several steps *)
+            exists (i2', i1'); exists s3'; split.
+            left; eauto.
+            eexists (_, _), (_, _). repeat split; eauto.
+            econstructor; eauto.
+          -- (* L3 makes no step *)
+            exists (i2', i1'); exists s3; split.
+            right; split. subst t; apply star_refl. red. left. auto.
+            eexists (_, _), (_, _). repeat split; eauto.
+            econstructor; eauto.
+        * (* L2 makes no step *)
+          exists (i2, i1'); exists s3; split.
+          right; split. subst t; apply star_refl. red. right. auto.
+            eexists (_, _), (_, _). repeat split; eauto. 1-2: reflexivity.
+            econstructor; eauto.
+    - unfold ff_order.
+      apply wf_lex_ord. apply Transitive_Closure.wf_clos_trans.
+      eapply (ST.fsim_order_wf H2). eapply (ST.fsim_order_wf H1).
+  Qed.
+
+End COMP_FSIM.
+
+Lemma st_fsim_vcomp
+  `(ccA1: ST.callconv liAs liAn) `(ccA2: ST.callconv liAn liAf)
+  `(ccB1: ST.callconv liBs liBn) `(ccB2: ST.callconv liBn liBf)
+  (Ls: semantics liAs liBs) (Ln: semantics liAn liBn) (Lf: semantics liAf liBf):
+  ST.forward_simulation ccA1 ccB1 Ls Ln ->
+  ST.forward_simulation ccA2 ccB2 Ln Lf ->
+  ST.forward_simulation (ST.cc_compose ccA1 ccA2) (ST.cc_compose ccB1 ccB2) Ls Lf.
+Proof.
+  intros [X] [Y]. constructor. eapply st_fsim_vcomp'; eauto.
+Qed.
+
+(** ** Left and Right Unit Laws *)
+
+Section ID_FSIM.
+
+  Context `(cc: ST.callconv liA liB) (sk: AST.program unit unit).
+  Inductive sf_ms: ST.ccworld cc ->  ST.ccworld cc ->
+                   @state liA _ (id_semantics sk) ->
+                   @state liB _ (id_semantics sk) -> Prop :=
+  | sf_ms_q w q1 q2:
+    ST.match_query cc w q1 q2 -> sf_ms w w (st_q q1) (st_q q2)
+  | sf_ms_r w r1 r2:
+    ST.match_reply cc w r1 r2 -> sf_ms w w (st_r r1) (st_r r2).
+
+  Lemma id_self_fsim :
+    ST.forward_simulation cc cc (id_semantics sk) (id_semantics sk).
+  Proof.
+    constructor.
+    eapply ST.Forward_simulation with (ltof _ (fun (_:unit) => 0))
+                                      (fun _ wa wb _ s1 s2 => sf_ms wa wb s1 s2)
+                                      (fun w1 w2 => w1 :-> w2); try reflexivity.
+    - intros. etransitivity; eauto.
+    - intros wa wb se Hw. constructor.
+      + intros q1 q2 s1 wb1 Hb Hq H. inv H. exists tt.
+        eexists. split. constructor.
+        exists wb1, wb1. repeat split; try easy.
+        etransitivity; eauto. now constructor.
+      + intros wa1 wb1 [] s1 s2 r1 Hs H. inv H. inv Hs.
+        eexists. split. constructor.
+        exists wb1. repeat split; easy.
+      + intros wa1 wb1 [] s1 s2 q1 Hs H. inv H. inv Hs.
+        eexists. split. constructor.
+        exists wb1. split. reflexivity. split. apply H2.
+        intros r1 r2 s1' wb2 Hb Hr H. inv H.
+        eexists tt, _. split. constructor.
+        exists wb2, wb2. repeat split; eauto. reflexivity.
+        now constructor.
+      + intros. easy.
+    - apply well_founded_ltof.
+  Qed.
+
+End ID_FSIM.
+
+Section CAT_SIM.
+
+  Lemma st_normalize_fsim `(ccA: ST.callconv liA1 liA2)
+        `(ccB: ST.callconv liB1 liB2) L1 L2:
+    ST.forward_simulation ccA ccB L1 L2 ->
+    STCAT.forward_simulation ccA ccB L1 L2.
+  Proof.
+    intros H. unfold STCAT.forward_simulation, normalize_sem.
+    assert (Hsk: skel L1 = skel L2).
+    { destruct H. apply (ST.fsim_skel X). }
+    unfold left_comp_id, right_comp_id. rewrite Hsk.
+    eapply st_fsim_lcomp_sk.
+    - apply id_self_fsim.
+    - eapply st_fsim_lcomp_sk.
+      + exact H.
+      + apply id_self_fsim.
+      + rewrite Hsk. apply Linking.linkorder_refl.
+      + rewrite <- Hsk. apply CategoricalComp.id_skel_order.
+    - apply CategoricalComp.id_skel_order.
+    - apply Linking.linkorder_refl.
+  Qed.
+
+  Lemma st_fsim_left_unit1 `(L: semantics liA liB):
+    STCAT.forward_simulation &1 &1 L (1 o L).
+  Proof. apply fsim_embed. apply CAT.left_unit_1. Qed.
+
+  Lemma st_fsim_left_unit2 `(L: semantics liA liB):
+    STCAT.forward_simulation &1 &1 (1 o L) L.
+  Proof. apply fsim_embed. apply CAT.left_unit_2. Qed.
+
+  Lemma st_fsim_right_unit1 `(L: semantics liA liB):
+    STCAT.forward_simulation &1 &1 L (L o 1).
+  Proof. apply fsim_embed. apply CAT.right_unit_1. Qed.
+
+  Lemma st_fsim_right_unit2 `(L: semantics liA liB):
+    STCAT.forward_simulation &1 &1 (L o 1) L.
+  Proof. apply fsim_embed. apply CAT.right_unit_2. Qed.
+
+  Section CC_UNIT.
+    Context `(ccA: ST.callconv liA1 liA2) `(ccB: ST.callconv liB1 liB2).
+    Lemma cc_right_unit L1 L2:
+      ST.forward_simulation (ST.cc_compose ccA &1) (ST.cc_compose ccB &1) L1 L2 ->
+      ST.forward_simulation ccA ccB L1 L2.
+    Proof.
+      intros [X]. constructor.
+      eapply ST.Forward_simulation with
+        (ST.fsim_order X)
+        (fun se w1 w2 => ST.fsim_match_states X se (w1, tt) (w2, tt))
+        (fun w1 w2 => ST.fsim_invariant X (w1, tt) (w2, tt)); try apply X.
+      intros. eapply ST.fsim_invariant_env_step; eauto. split; easy.
+      intros wa wb se HI.
+      pose proof (ST.fsim_lts X (wa, tt) (wb, tt) se HI) as H.
+      constructor.
+      - intros. exploit @ST.fsim_match_initial_states; eauto.
+        instantiate (1 := (_, _)). split; eauto. reflexivity.
+        econstructor. split; try easy. eauto.
+        intros. cbn in *. eprod_crush. repeat esplit; eauto.
+      - intros. exploit @ST.fsim_match_final_states; eauto.
+        intros. cbn in *. eprod_crush. subst. repeat esplit; eauto.
+      - intros. exploit @ST.fsim_match_external; eauto.
+        intros. cbn in *. eprod_crush. subst.
+        eexists. repeat split; eauto. eexists; repeat split; eauto.
+        intros. exploit H5; eauto. instantiate (1 := (_, _)).
+        split; eauto. cbn. repeat esplit; eauto.
+        intros. cbn in *. eprod_crush. repeat esplit; eauto.
+      - intros. exploit @ST.fsim_simulation; eauto.
+        intros. cbn in *. eprod_crush. repeat esplit; eauto.
+        Unshelve. exact tt.
+    Qed.
+    Lemma cc_left_unit L1 L2:
+      ST.forward_simulation (ST.cc_compose &1 ccA) (ST.cc_compose &1 ccB) L1 L2 ->
+      ST.forward_simulation ccA ccB L1 L2.
+    Proof.
+      intros [X]. constructor.
+      eapply ST.Forward_simulation with
+        (ST.fsim_order X)
+        (fun se w1 w2 => ST.fsim_match_states X se (tt, w1) (tt, w2))
+        (fun w1 w2 => ST.fsim_invariant X (tt, w1) (tt, w2)); try apply X.
+      intros. eapply ST.fsim_invariant_env_step; eauto. split; easy.
+      intros wa wb se HI.
+      pose proof (ST.fsim_lts X (tt, wa) (tt, wb) se HI) as H.
+      constructor.
+      - intros. exploit @ST.fsim_match_initial_states; eauto.
+        instantiate (1 := (_, _)). split; eauto. reflexivity.
+        econstructor. split; try easy. eauto.
+        intros. cbn in *. eprod_crush. repeat esplit; eauto.
+      - intros. exploit @ST.fsim_match_final_states; eauto.
+        intros. cbn in *. eprod_crush. subst. repeat esplit; eauto.
+      - intros. exploit @ST.fsim_match_external; eauto.
+        intros. cbn in *. eprod_crush. subst.
+        eexists. repeat split; eauto. eexists; repeat split; eauto.
+        intros. exploit H5; eauto. instantiate (1 := (_, _)).
+        split; eauto. cbn. repeat esplit; eauto.
+        intros. cbn in *. eprod_crush. repeat esplit; eauto.
+      - intros. exploit @ST.fsim_simulation; eauto.
+        intros. cbn in *. eprod_crush. repeat esplit; eauto.
+        Unshelve. exact tt.
+    Qed.
+  End CC_UNIT.
+
+  Lemma st_cat_fsim_lcomp_sk
+        `(ccA: ST.callconv liA1 liA2)
+        `(ccB: ST.callconv liB1 liB2)
+        `(ccC: ST.callconv liC1 liC2)
+        L1s L2s L1t L2t sk:
+    STCAT.forward_simulation ccB ccC L1s L1t ->
+    STCAT.forward_simulation ccA ccB L2s L2t ->
+    Linking.linkorder (skel L1s) sk ->
+    Linking.linkorder (skel L2s) sk ->
+    STCAT.forward_simulation ccA ccC
+                             (comp_semantics' L1s L2s sk)
+                             (comp_semantics' L1t L2t sk).
+  Proof.
+    intros X Y HSK1 HSK2. exploit @st_fsim_lcomp_sk.
+    apply X. apply Y. apply HSK1. apply HSK2. intros Z. clear X Y.
+    unfold STCAT.forward_simulation.
+    assert (HX: ST.forward_simulation
+                &1 &1 (normalize_sem (comp_semantics' L1s L2s sk))
+                      (comp_semantics' (normalize_sem L1s) (normalize_sem L2s) sk)).
+    { apply fsim_embed. apply normalize_comp_fsim_sk1. }
+    assert (HY: ST.forward_simulation
+                &1 &1 (comp_semantics' (normalize_sem L1t) (normalize_sem L2t) sk)
+                      (normalize_sem (comp_semantics' L1t L2t sk))).
+    { apply fsim_embed. apply normalize_comp_fsim_sk2. }
+    exploit @st_fsim_vcomp. apply HX. apply Z. intros HZ. clear HX Z.
+    exploit @st_fsim_vcomp. apply HZ. apply HY. intros H. clear HZ HY.
+    apply cc_left_unit. apply cc_right_unit. apply H.
+  Qed.
+
+End CAT_SIM.
+
+(** ** Refinement between Stateful Simulation Conventions *)
+
+Definition st_ccref {li1 li2} (cc1 cc2: ST.callconv li1 li2) : Prop :=
+  STCAT.forward_simulation cc2 cc1 1 1.
+
+(** A simplified condition for sim. conv. refinement given the situation that
+    their states are isomorphic *)
+Section CCREF.
+
+  Context {li1 li2} (ccA ccB: ST.callconv li1 li2).
+
+  Variable F: ST.ccworld ccA -> ST.ccworld ccB.
+  Variable G: ST.ccworld ccB -> ST.ccworld ccA.
+  Hypothesis F_init: F (@pset_init (ST.ccworld ccA) _) = @pset_init (ST.ccworld ccB) _.
+  Hypothesis F_ext_step: forall x y, F x :-> F y -> x :-> y.
+  Hypothesis F_int_step: forall x y, x *-> y -> F x *-> F y.
+  Hypothesis FG_cancel: forall x, F (G x) = x.
+  Hypothesis F_mq:
+    forall wa q1 q2, ST.match_query ccB (F wa) q1 q2 -> ST.match_query ccA wa q1 q2.
+  Hypothesis F_mr:
+    forall wa r1 r2, ST.match_reply ccA wa r1 r2 -> ST.match_reply ccB (F wa) r1 r2.
+
+  Inductive cc_inv: ST.ccworld ccA -> ST.ccworld ccB -> Prop :=
+  | cc_inv_intro wa wb: F wa :-> wb -> cc_inv wa wb.
+  Inductive cc_ms: ST.ccworld ccA -> ST.ccworld ccB -> @state li1 li1 1 -> @state li2 li2 1 -> Prop :=
+  | cc_ms_q q1 q2 wa wb:
+    F wa = wb -> ST.match_query ccB wb q1 q2 -> cc_ms wa wb (st_q q1) (st_q q2)
+  | cc_ms_r r1 r2 wa wb:
+    F wa = wb -> ST.match_reply ccB wb r1 r2 -> cc_ms wa wb (st_r r1) (st_r r2).
+
+  Lemma st_ccref_intro: st_ccref ccB ccA.
+  Proof.
+    apply st_normalize_fsim. constructor.
+    eapply ST.Forward_simulation with
+      (ltof _ (fun (_: unit) => 0)) (fun _ wa wb _ => cc_ms wa wb)
+      (fun wa wb => cc_inv wa wb); try easy.
+    - intros. inv H. constructor. etransitivity; eauto.
+    - constructor. rewrite F_init. reflexivity.
+    - intros wa wb se I. inv I.
+      constructor.
+      + intros q1 q2 s1 wb1 Hb Hq Hx. exists tt. inv Hx. exists (st_q q2).
+        split. constructor.
+        exists (G wb1), wb1. repeat split; try easy.
+        * apply F_ext_step. rewrite FG_cancel.
+          etransitivity; eauto.
+        * constructor. apply FG_cancel. apply Hq.
+      + intros wa1 wb1 [] s1 s2 r1 Hs Hx. inv Hx.
+        inv Hs. exists r2. split. constructor.
+        exists (F wa1). repeat split; easy.
+      + intros wa1 wb1 [] s1 s2 q1 Hs Hx. inv Hx. inv Hs.
+        exists q2. split. constructor.
+        exists wa1. split. reflexivity. split. eauto.
+        intros r1 r2 s1' wa2 Ha2 Hr Hy.
+        inv Hy. eexists tt, _. split. constructor.
+        eexists wa2, (F wa2). repeat split; try easy.
+        apply F_int_step. assumption.
+        constructor; eauto.
+      + intros. easy.
+  Qed.
+
+End CCREF.
+
+(** ** Left and Right Unit Laws for Sim. Conv. *)
+
+Section CC_UNIT.
+
+  Context `(cc: ST.callconv liA liB).
+
+  Inductive lu_inv: ST.ccworld cc -> ST.ccworld cc -> Prop :=
+  | lu_inv_intro wa wb:
+    wa :-> wb -> lu_inv wa wb.
+  Inductive lu_ms: ST.ccworld cc -> ST.ccworld cc -> @state liA liA 1 -> @state liB liB 1 -> Prop :=
+  | lu_ms_q w q1 q2:
+    ST.match_query cc w q1 q2 -> lu_ms w w (st_q q1) (st_q q2)
+  | lu_ms_r w r1 r2:
+    ST.match_reply cc w r1 r2 -> lu_ms w w (st_r r1) (st_r r2).
+
+  Lemma ccref_left_unit1:
+    st_ccref cc (ST.cc_compose &1 cc).
+  Proof.
+    unfold st_ccref. apply st_normalize_fsim. constructor.
+    eapply ST.Forward_simulation with
+      (ltof _ (fun (_: unit) => 0)) (fun _ '(_, w1) w2 _ => lu_ms w1 w2)
+      (fun '(_, w1) w2 => lu_inv w1 w2); try easy.
+    - intros [? wa] wb I wb1 Hb. inv I.
+      constructor. etransitivity; eauto.
+    - intros [? wa] wb se I. constructor.
+      + intros q1 q2 s1 wb1 Hb Hq H. inv H. exists tt, (st_q q2).
+        split. constructor.
+        exists (tt, wb1), wb1. repeat split; try easy.
+        inv I. etransitivity; eauto.
+        constructor. eauto.
+      + intros [? wa1] wb1 [] s1 s2 r1 Hs H. inv H. inv Hs.
+        exists r2. split. constructor.
+        exists wb1. repeat split; easy.
+      + intros [? wa1] wb1 [] s1 s2 q1 Hs H. inv H. inv Hs.
+        exists q2. split. constructor.
+        exists (tt, wb1). repeat split; try easy.
+        eexists. split; eauto. reflexivity.
+        intros r1 r2 s1' [? wa2] [? Ha] Hr HX.
+        destruct Hr as (x & HR1 & HR2).
+        inv HR1. inv HX.
+        exists tt, (st_r r2). repeat split.
+        exists (tt, wa2), wa2.
+        repeat split; eauto. destruct c. reflexivity.
+        constructor. assumption.
+      + intros. easy.
+  Qed.
+
+  Lemma ccref_left_unit2:
+    st_ccref (ST.cc_compose &1 cc) cc.
+  Proof.
+    unfold st_ccref. apply st_normalize_fsim. constructor.
+    eapply ST.Forward_simulation with
+      (ltof _ (fun (_: unit) => 0)) (fun _ w1 '(_, w2) _ => lu_ms w1 w2)
+      (fun w1 '(_, w2) => lu_inv w1 w2); try easy.
+    - intros wa [? wb] I [? wb1] [? Hb]. inv I.
+      constructor. etransitivity; eauto.
+    - intros wa [? wb] se I. constructor.
+      + intros q1 q2 s1 [? wb1] [_ Hb] Hq H. inv H. exists tt, (st_q q2).
+        split. constructor.
+        destruct Hq as (x & HQ1 & HQ2).
+        inv HQ1.
+        eexists wb1, (tt, wb1). repeat split; try easy.
+        inv I. etransitivity; eauto.
+        1-2: constructor; eauto.
+      + intros wa1 [? wb1] [] s1 s2 r1 Hs H. inv H. inv Hs.
+        exists r2. split. constructor.
+        eexists (tt, wb1). repeat split; try easy.
+        eexists; split; eauto. reflexivity.
+      + intros wa1 [? wb1] [] s1 s2 q1 Hs H. inv H. inv Hs.
+        exists q2. split. constructor.
+        exists wb1. repeat split; try easy.
+        intros r1 r2 s1' wa2 Ha Hr HX. inv HX.
+        exists tt, (st_r r2). repeat split.
+        exists wa2, (tt, wa2).
+        repeat split; eauto. reflexivity.
+        constructor. assumption.
+      + intros. easy.
+  Qed.
+
+  Lemma ccref_right_unit1:
+    st_ccref cc (ST.cc_compose cc &1).
+  Proof.
+  Proof.
+    unfold st_ccref. apply st_normalize_fsim. constructor.
+    eapply ST.Forward_simulation with
+      (ltof _ (fun (_: unit) => 0)) (fun _ '(w1, _) w2 _ => lu_ms w1 w2)
+      (fun '(w1, _) w2 => lu_inv w1 w2); try easy.
+    - intros [wa _] wb I wb1 Hb. inv I.
+      constructor. etransitivity; eauto.
+    - intros [wa ?] wb se I. constructor.
+      + intros q1 q2 s1 wb1 Hb Hq H. inv H. exists tt, (st_q q2).
+        split. constructor.
+        exists (wb1, tt), wb1. repeat split; try easy.
+        inv I. etransitivity; eauto.
+        constructor. eauto.
+      + intros [wa1 ?] wb1 [] s1 s2 r1 Hs H. inv H. inv Hs.
+        exists r2. split. constructor.
+        exists wb1. repeat split; easy.
+      + intros [wa1 ?] wb1 [] s1 s2 q1 Hs H. inv H. inv Hs.
+        exists q2. split. constructor.
+        exists (wb1, tt). repeat split; try easy.
+        eexists. split; eauto. reflexivity.
+        intros r1 r2 s1' [wa2 ?] [Ha ?] Hr HX.
+        destruct Hr as (x & HR1 & HR2).
+        inv HR2. inv HX.
+        exists tt, (st_r r2). repeat split.
+        exists (wa2, tt), wa2.
+        repeat split; eauto. reflexivity. destruct c.
+        constructor. assumption.
+      + intros. easy.
+  Qed.
+
+  Lemma ccref_right_unit2:
+    st_ccref (ST.cc_compose cc &1) cc.
+  Proof.
+    unfold st_ccref. apply st_normalize_fsim. constructor.
+    eapply ST.Forward_simulation with
+      (ltof _ (fun (_: unit) => 0)) (fun _ w1 '(w2, _) _ => lu_ms w1 w2)
+      (fun w1 '(w2, _) => lu_inv w1 w2); try easy.
+    - intros wa [wb ?] I [wb1 ?] [Hb ?]. inv I.
+      constructor. etransitivity; eauto.
+    - intros wa [wb ?] se I. constructor.
+      + intros q1 q2 s1 [wb1 ?] [Hb _] Hq H. inv H. exists tt, (st_q q2).
+        split. constructor.
+        destruct Hq as (x & HQ1 & HQ2).
+        inv HQ2.
+        eexists wb1, (wb1, tt). repeat split; try easy.
+        inv I. etransitivity; eauto.
+        all: constructor; eauto.
+      + intros wa1 [wb1 ?] [] s1 s2 r1 Hs H. inv H. inv Hs.
+        exists r2. split. constructor.
+        eexists (wb1, tt). repeat split; try easy.
+        eexists; split; eauto. reflexivity.
+      + intros wa1 [wb1 ?] [] s1 s2 q1 Hs H. inv H. inv Hs.
+        exists q2. split. constructor.
+        exists wb1. repeat split; try easy.
+        intros r1 r2 s1' wa2 Ha Hr HX. inv HX.
+        exists tt, (st_r r2). repeat split.
+        exists wa2, (wa2, tt).
+        repeat split; eauto. reflexivity.
+        constructor. assumption.
+      + intros. easy.
+  Qed.
+
+End CC_UNIT.
+
+(** ** Monotonicity of Sim. Conv. *)
+
+Require Import LogicalRelations.
+
+Instance st_fsim_preo {li1 li2}:
+  PreOrder (ST.forward_simulation &(@cc_id li1) &(@cc_id li2)).
+Proof.
+  split.
+  - intros L. apply fsim_embed. reflexivity.
+  - intros L1 L2 L3 H12 H23.
+    exploit @st_fsim_vcomp. apply H12. apply H23.
+    intros H. apply cc_right_unit. apply H.
+Qed.
+
+Instance st_fsim_proper `(ccA: ST.callconv liA1 liA2) `(ccB: ST.callconv liB1 liB2):
+  Proper ((ST.forward_simulation &1 &1) --> (ST.forward_simulation &1 &1) ++> impl)
+         (ST.forward_simulation ccA ccB).
+Proof.
+  intros X Y HXY A B HAB HL.
+  exploit @st_fsim_vcomp. exact HXY. exact HL. intros HL'.
+  exploit @st_fsim_vcomp. exact HL'. exact HAB. intros HL''.
+  apply (cc_left_unit (cc_right_unit HL'')).
+Qed.
+
+Global Instance ccref_preo li1 li2:
+  PreOrder (@st_ccref li1 li2).
+Proof.
+  split.
+  - intros cc. eapply st_ccref_intro with id id; try easy.
+  - intros cc1 cc2 cc3 H12 H23.
+    unfold st_ccref in *.
+    exploit @st_fsim_lcomp_sk. apply H12. apply H23.
+    1-2: apply Linking.linkorder_refl. cbn. intros X.
+    match type of X with
+    | ST.forward_simulation _ _ ?x ?y =>
+        set (LX := x); set (LY := y)
+    end.
+    assert (Y: forward_simulation 1 1 (normalize_sem 1) LX).
+    {
+      subst LX.
+      etransitivity. 2: apply assoc1.
+      etransitivity. apply CAT.right_unit_1.
+      etransitivity. apply CAT.right_unit_1.
+      etransitivity. apply CAT.right_unit_1.
+      eapply categorical_compose_simulation'. reflexivity.
+      etransitivity. 2: apply assoc2.
+      etransitivity. 2: apply assoc2.
+      eapply categorical_compose_simulation'. 2: reflexivity.
+      eapply categorical_compose_simulation'. 2: reflexivity.
+      eapply categorical_compose_simulation'. 1-2: reflexivity.
+      all: apply Linking.linkorder_refl.
+    }
+    assert (Z: forward_simulation 1 1 LY (normalize_sem 1)).
+    {
+      subst LY.
+      etransitivity. 2: apply CAT.right_unit_2.
+      etransitivity. 2: apply CAT.right_unit_2.
+      etransitivity. 2: apply CAT.right_unit_2.
+      etransitivity. apply assoc2.
+      eapply categorical_compose_simulation'. reflexivity.
+      etransitivity. apply assoc1.
+      etransitivity. apply assoc1.
+      eapply categorical_compose_simulation'. 2: reflexivity.
+      eapply categorical_compose_simulation'. 2: reflexivity.
+      eapply categorical_compose_simulation'. 1-2: reflexivity.
+      all: apply Linking.linkorder_refl.
+    }
+    unfold STCAT.forward_simulation.
+    rewrite -> (fsim_embed Y). rewrite <- (fsim_embed Z). apply X.
+Qed.
+
+Global Instance st_fsim_ccref:
+  Monotonic
+    (@STCAT.forward_simulation)
+    (forallr - @ liA1, forallr - @ liA2, st_ccref ++>
+     forallr - @ liB1, forallr - @ liB2, st_ccref -->
+     subrel).
+Proof.
+  intros liA1 liA2 ccA1 ccA2 HA
+         liB1 liB2 ccB1 ccB2 HB L1 L2 H.
+  assert (Hsk: skel L1 = skel L2).
+  { destruct H. apply X. }
+  unfold flip, st_ccref in *.
+  exploit @st_cat_fsim_lcomp_sk. exact H. exact HA.
+  apply Linking.linkorder_refl. apply CategoricalComp.id_skel_order.
+  intros HC.
+  exploit @st_cat_fsim_lcomp_sk. exact HB. exact HC.
+  apply CategoricalComp.id_skel_order. apply Linking.linkorder_refl.
+  cbn. intros X. rewrite Hsk in X at 3 4. clear -X.
+  assert (Y: STCAT.forward_simulation &1 &1 L1 (1 o L1 o 1)).
+  {
+    exploit @st_fsim_vcomp.
+    apply st_fsim_right_unit1. apply st_fsim_left_unit1.
+    apply cc_left_unit.
+  }
+  assert (Z: STCAT.forward_simulation &1 &1 (1 o L2 o 1) L2).
+  {
+    exploit @st_fsim_vcomp.
+    apply st_fsim_left_unit2. apply st_fsim_right_unit2.
+    apply cc_left_unit.
+  }
+  exploit @st_fsim_vcomp. exact Y. exact X. clear Y X. intros W.
+  exploit @st_fsim_vcomp. exact W. exact Z. clear W Z. intros X.
+  apply (cc_left_unit (cc_right_unit X)).
+Qed.
+
+(** * Encapsulation Properties *)
+
+(** ** Composition of Components with Encapsulated States *)
+
+Section LI_FUNC.
+
+  Program Definition callconv_map
+          `(F: LiIso liA1 liX1) `(G: LiIso liB1 liY1) cc : callconv liX1 liY1 :=
+    {|
+      ccworld := ccworld cc;
+      match_query w q1 q2 := match_query cc w (fq F q1) (fq G q2);
+      match_reply w r1 r2 :=
+        exists r1' r2', r1 = fr F r1' /\ r2 = fr G r2' /\ match_reply cc w r1' r2';
+      match_senv := match_senv cc;
+    |}.
+  Next Obligation. eauto using match_senv_public_preserved. Qed.
+  Next Obligation. eauto using match_senv_valid_for. Qed.
+  Next Obligation. (* Admitted *). eauto using match_senv_symbol_address. Qed.
+  Next Obligation. (* Admitted. *) eauto using match_query_defined. Qed.
+
+  Program Definition st_callconv_map
+          `(F: LiIso liA1 liX1) `(G: LiIso liB1 liY1) cc : ST.callconv liX1 liY1 :=
+    {|
+      ST.ccworld := ST.ccworld cc;
+      ST.match_query w q1 q2 := ST.match_query cc w (fq F q1) (fq G q2);
+      ST.match_reply w r1 r2 :=
+        exists r1' r2', r1 = fr F r1' /\ r2 = fr G r2' /\
+                     ST.match_reply cc w r1' r2';
+    |}.
+
+  Context `(F1: LiIso liA1 liX1) `(G1: LiIso liB1 liY1)
+          `(F2: LiIso liA2 liX2) `(G2: LiIso liB2 liY2).
+
+  Section NO_STATE.
+    Context (cc1: callconv liA1 liB1) (cc2: callconv liA2 liB2).
+    Lemma map_monotonicity_cc L1 L2:
+      forward_simulation cc1 cc2 L1 L2 ->
+      forward_simulation (callconv_map F1 G1 cc1) (callconv_map F2 G2 cc2)
+                         (semantics_map L1 F1 F2) (semantics_map L2 G1 G2).
+    Proof.
+      intros [[]]. constructor. econstructor; eauto.
+      instantiate (1 := fsim_match_states).
+      intros. exploit fsim_lts; eauto.
+      intros HL. constructor.
+      - intros. cbn in *.
+        exploit @fsim_match_initial_states; eauto.
+      - intros. cbn in *. eprod_crush. subst.
+        exploit @fsim_match_final_states; eauto.
+        intros X. eprod_crush.
+        eexists. repeat split; eauto.
+      - intros. cbn in *.
+        exploit @fsim_match_external; eauto.
+        intros. eprod_crush.
+        edestruct (@fq_surj _ _ G1 x0). subst.
+        eexists x, _. repeat split; eauto.
+        intros. eprod_crush. subst.
+        eapply fr_inj in H8. subst.
+        exploit @H6; eauto. intros. eprod_crush.
+        eexists _, _. repeat split; eauto.
+      - intros. exploit @fsim_simulation; eauto.
+    Qed.
+  End NO_STATE.
+
+  Section STATE.
+    Context (cc1: ST.callconv liA1 liB1) (cc2: ST.callconv liA2 liB2).
+    Lemma st_map_monotonicity_cc L1 L2:
+      ST.forward_simulation cc1 cc2 L1 L2 ->
+      ST.forward_simulation (st_callconv_map F1 G1 cc1) (st_callconv_map F2 G2 cc2)
+                            (semantics_map L1 F1 F2) (semantics_map L2 G1 G2).
+    Proof.
+      intros [[]]. constructor. econstructor; eauto.
+      instantiate (1 := fsim_match_states).
+      intros. exploit fsim_lts; eauto. clear.
+      intros HL. constructor.
+      - intros. cbn in H1, H2.
+        exploit @ST.fsim_match_initial_states; eauto.
+      - intros. cbn in *. eprod_crush. subst.
+        exploit @ST.fsim_match_final_states; eauto.
+        intros X. eprod_crush.
+        eexists. repeat split; eauto.
+        eexists. repeat split; eauto.
+      - intros. cbn in *.
+        exploit @ST.fsim_match_external; eauto.
+        intros. eprod_crush.
+        edestruct (@fq_surj _ _ G1 x). subst.
+        eexists. repeat split; eauto.
+        eexists. repeat split; eauto.
+        intros. eprod_crush. subst.
+        eapply fr_inj in H8. subst.
+        exploit @H5; eauto. intros. eprod_crush.
+        eexists _, _. repeat split; eauto.
+      - intros. exploit @ST.fsim_simulation; eauto.
+    Qed.
+  End STATE.
+
+End LI_FUNC.
+
+(* TODO: move to somewhere else *)
+Section MAP_NORMALIZE.
+
+  Context `(F: LiIso liA1 liA2) `(G: LiIso liB1 liB2) (L : semantics liA1 liB1).
+
+  Inductive mn_ms: state (normalize_sem $L) -> state $(normalize_sem L) -> Prop :=
+  | mn_ms1 q1 q2:
+    fq G q1 = q2 -> mn_ms (st1 1 _ (st_q q1)) (st1 1 _ (st_q q2))
+  | mn_ms2 q1 q2 s:
+    fq G q1 = q2 ->
+    mn_ms (st2 1 ((semantics_map L F G) o 1) (st_q q1) (st1 (semantics_map L F G) _ s))
+          (st2 1 (L o 1) (st_q q2) (st1 L _ s))
+  | mn_ms3 q1 q2 s q3 q4:
+    fq G q1 = q2 -> fq F q3 = q4 ->
+    mn_ms (st2 1 ((semantics_map L F G) o 1) (st_q q1) (st2 (semantics_map L F G) 1 s (st_q q3)))
+          (st2 1 (L o 1) (st_q q2) (st2 L 1 s (st_q q4)))
+  | mn_ms4 q1 q2 s r1 r2:
+    fq G q1 = q2 -> fr F r2 = r1 ->
+    mn_ms (st2 1 ((semantics_map L F G) o 1) (st_q q1) (st2 (semantics_map L F G) 1 s (st_r r1)))
+          (st2 1 (L o 1) (st_q q2) (st2 L 1 s (st_r r2)))
+  | mn_ms5 r1 r2:
+    fr G r2 = r1 -> mn_ms (st1 1 _ (st_r r1)) (st1 1 _ (st_r r2)).
+
+  Lemma map_normalize1:
+    forward_simulation 1 1 (normalize_sem $L) $(normalize_sem L).
+  Proof.
+    constructor. econstructor.
+    reflexivity. firstorder.
+    intros. inv H.
+    eapply forward_simulation_step with (match_states := mn_ms).
+    - intros q ? s1 [] H. inv H. inv H1.
+      eexists. split; repeat constructor.
+    - intros s1 s2 r1 Hs H. inv H. inv H1. inv Hs.
+      eexists. split; repeat constructor.
+      eexists. repeat split; eauto.
+    - intros s1 s2 q1 Hs H. exists tt. inv H. inv H1. inv H. inv Hs.
+      eexists. repeat split.
+      intros r ? s1' [] H. inv H. inv H5. inv H4.
+      edestruct (@fr_surj _ _ F r). subst.
+      eexists. repeat split; eauto.
+      eexists; repeat split; eauto.
+      constructor; reflexivity.
+    - intros * HSTEP * HS. inv HS.
+      + inv HSTEP. inv H1. inv H1. inv H2.
+        eexists; split.
+        eapply step_push; constructor; eauto. apply H.
+        constructor; reflexivity.
+      + inv HSTEP. inv H4.
+        * eexists; split.
+          apply step2. apply step1. apply H1.
+          constructor; reflexivity.
+        * inv H2. eexists; split.
+          eapply step2. eapply step_push. apply H1. constructor.
+          constructor; easy.
+        * inv H2. inv H5. cbn in *. eprod_crush. subst.
+          eexists; split.
+          eapply step_pop; constructor. apply H1.
+          constructor; easy.
+      + inv HSTEP. inv H4. inv H5. inv H2. inv H2.
+      + inv HSTEP. inv H4. inv H5. 2: inv H2. inv H2.
+        cbn in *. eprod_crush. eapply fr_inj in H. subst.
+        eexists. split. apply step2. eapply step_pop.
+        constructor. eauto. constructor; easy.
+      + inv HSTEP. inv H1. inv H1.
+    - apply well_founded_ltof.
+  Qed.
+
+  Lemma map_normalize2:
+    forward_simulation 1 1 $(normalize_sem L) (normalize_sem $L).
+  Proof.
+    constructor. econstructor.
+    reflexivity. firstorder.
+    intros. inv H.
+    eapply forward_simulation_step with (match_states := flip mn_ms).
+    - intros q ? s1 [] H. inv H. inv H1.
+      eexists. split; repeat constructor.
+    - intros s1 s2 r1 Hs H. inv H. inv H1. inv H2. inv H. inv Hs.
+      eexists. split; repeat constructor.
+    - intros s1 s2 q1 Hs H. exists tt. inv H. inv H1. inv H. inv Hs.
+      apply fq_inj in H5. subst.
+      eexists. repeat split.
+      intros. inv H. cbn in *. eprod_crush. subst.
+      inv H1. inv H5. inv H4.
+      eexists. repeat split. constructor; reflexivity.
+    - intros * HSTEP * HS. inv HS.
+      + inv HSTEP. inv H1. inv H1. inv H2.
+        eexists; split.
+        eapply step_push; constructor; eauto. apply H.
+        constructor; reflexivity.
+      + inv HSTEP. inv H4.
+        * eexists; split.
+          apply step2. apply step1. apply H1.
+          constructor; reflexivity.
+        * inv H2. edestruct (@fq_surj _ _ F q). subst.
+          eexists; split. eapply step2. eapply step_push.
+          apply H1. constructor.
+          constructor; easy.
+        * inv H2. inv H5.
+          eexists; split. eapply step_pop; constructor.
+          eexists; split; eauto. constructor; easy.
+      + inv HSTEP. inv H4. inv H5. inv H2. inv H2.
+      + inv HSTEP. inv H4. inv H5. 2: inv H2. inv H2.
+        eexists. split.
+        apply step2. eapply step_pop. constructor.
+        eexists; split; eauto.
+        constructor; easy.
+      + inv HSTEP. inv H1. inv H1.
+    - apply well_founded_ltof.
+  Qed.
+
+End MAP_NORMALIZE.
+
+Require Import FunctionalExtensionality.
+Require Import PropExtensionality.
+
+Lemma st_cc_map_id `(cc: ST.callconv liA liB):
+  st_callconv_map li_iso_id li_iso_id cc = cc.
+Proof.
+  destruct cc. unfold st_callconv_map. cbn.
+  f_equal.
+  extensionality x. extensionality y. extensionality z.
+  apply propositional_extensionality.
+  split.
+  - intros. eprod_crush. subst. apply H1.
+  - intros. eexists _, _. repeat split; eauto.
+Qed.
+
+Lemma cc_map_id `(cc: callconv liA liB):
+  callconv_map li_iso_id li_iso_id cc = cc.
+Proof.
+  destruct cc. unfold callconv_map. cbn.
+  f_equal; try apply Axioms.proof_irr.
+  extensionality x. extensionality y. extensionality z.
+  apply propositional_extensionality.
+  split.
+  - intros. eprod_crush. subst. apply H1.
+  - intros. eexists _, _. repeat split; eauto.
+Qed.
+
+Lemma cc_lift_twice `{PSet S1} `{PSet S2} `{PSet T1} `{PSet T2} `(cc: ST.callconv liA liB):
+  st_ccref (ST.callconv_lift cc (S1 * S2) (T1 * T2))
+           (st_callconv_map lf lf (ST.callconv_lift (ST.callconv_lift cc S1 T1) S2 T2)).
+Proof.
+  match goal with
+  | |- st_ccref ?x ?y => set (w1 := ST.ccworld x); set (w2 := ST.ccworld y)
+  end.
+  set (F := fun '(((a, b, c), d, e): w2) => (a, (b, d), (c, e))).
+  set (G := fun '((a, (b, d), (c, e)): w1) => ((a, b, c), d, e)).
+  eapply st_ccref_intro with F G.
+  - reflexivity.
+  - intros x y Hxy. cbn in *. eprod_crush. cbn in *.
+    eprod_crush. repeat split; easy.
+  - intros x y Hyx. cbn in *. eprod_crush. cbn in *.
+    repeat split; easy.
+  - intros. cbn in *. eprod_crush. reflexivity.
+  - intros. cbn in *. eprod_crush. cbn in *.
+    eprod_crush. repeat split; easy.
+  - intros. cbn in *. eprod_crush. cbn in *.
+    eprod_crush. subst. repeat split; easy.
+Qed.
+
+Section LIFT_UNIT.
+
+  Context {li: language_interface} {S: Type}.
+  Inductive su_ms: @state (li@S) _ 1 ->
+                   @state (li@S) _ (1@S) -> Prop :=
+  | su_ms_q q s:
+    su_ms (@st_q (li@S) (q,s)) ((st_q q), s)
+  | su_ms_r r s:
+    su_ms (@st_r (li@S) (r,s)) ((st_r r), s).
+  Hint Constructors su_ms.
+  Lemma lift_unit1: forward_simulation (@cc_id (li@S)) 1 1 (1 @ S).
+  Proof.
+    constructor. econstructor.
+    reflexivity. firstorder.
+    intros. inv H.
+    apply forward_simulation_step with (match_states := su_ms).
+    - intros. inv H. inv H1. cbn in *. eprod_crush.
+      eexists (_, _). repeat split; eauto.
+    - intros. inv H1. inv H.
+      eexists (_, _). repeat split.
+    - intros. inv H1. inv H.
+      eexists tt, (_, _). repeat split.
+      intros. inv H. inv H1. cbn in *. eprod_crush.
+      eexists (_, _). repeat split; eauto.
+    - easy.
+    - apply well_founded_ltof.
+  Qed.
+
+  Lemma lift_unit2: forward_simulation (@cc_id (li@S)) 1 (1 @ S) 1.
+    constructor. econstructor.
+    reflexivity. firstorder.
+    intros. inv H.
+    apply forward_simulation_step with (match_states := flip su_ms).
+    - intros. inv H. inv H1. inv H. cbn in *. eprod_crush.
+      eexists. repeat split; eauto. constructor.
+    - intros. inv H1. inv H. inv H2. inv H2. cbn in *. eprod_crush.
+      eexists. repeat split.
+    - intros. inv H1. inv H. inv H2. cbn in *.  eprod_crush.
+      eexists tt, _. repeat split.
+      intros. inv H. inv H1. inv H. cbn in *. eprod_crush.
+      eexists. repeat split; eauto. constructor. inv H2.
+    - intros. cbn in *. eprod_crush. inv H.
+    - apply well_founded_ltof.
+  Qed.
+
+End LIFT_UNIT.
+
+(* TODO: move to Lifting.v *)
+Lemma fsim_lift_normalize1 {S} `(L: semantics liA liB):
+  forward_simulation 1 1 (normalize_sem (L @ S)) (normalize_sem L @ S).
+Proof.
+  setoid_rewrite <- lift_categorical_comp2.
+  eapply categorical_compose_simulation'.
+  apply lift_unit1.
+  setoid_rewrite <- lift_categorical_comp2.
+  eapply categorical_compose_simulation'.
+  reflexivity.
+  apply lift_unit1.
+  all: cbn; (apply Linking.linkorder_refl || apply CategoricalComp.id_skel_order).
+Qed.
+
+Lemma fsim_lift_normalize2 {S} `(L: semantics liA liB):
+  forward_simulation 1 1 (normalize_sem L @ S) (normalize_sem (L @ S)).
+Proof.
+  setoid_rewrite lift_categorical_comp1.
+  eapply categorical_compose_simulation'.
+  apply lift_unit2.
+  setoid_rewrite -> lift_categorical_comp1.
+  eapply categorical_compose_simulation'.
+  reflexivity.
+  apply lift_unit2.
+  all: cbn; (apply Linking.linkorder_refl || apply CategoricalComp.id_skel_order).
+Qed.
+
+Section COMP.
+  Context `(ccA: ST.callconv liA1 liA2)
+          `(ccB: ST.callconv liB1 liB2)
+          `(ccC: ST.callconv liC1 liC2)
+          (L1s: liB1 +-> liC1) (L2s: liA1 +-> liB1)
+          (L1t: liB2 +-> liC2) (L2t: liA2 +-> liB2).
+  Context (HL1: E.forward_simulation ccB ccC L1s L1t)
+          (HL2: E.forward_simulation ccA ccB L2s L2t)
+          sk (Hsk1: Linking.linkorder (skel L1s) sk)
+          (Hsk2: Linking.linkorder (skel L2s) sk).
+
+  Lemma encap_fsim_lcomp_sk:
+    E.forward_simulation ccA ccC (comp_esem' L1s L2s sk) (comp_esem' L1t L2t sk).
+  Proof.
+    unfold E.forward_simulation in *. unfold comp_esem in *.
+    eapply st_fsim_lift with (K1:=pstate L2s) (K2:=pstate L2t) in HL1.
+    exploit @st_fsim_lcomp_sk. exact HL1. exact HL2. 1-2: eauto.
+    intros X. cbn. rewrite cc_lift_twice.
+    unfold STCAT.forward_simulation.
+    rewrite (fsim_embed (map_normalize1 _ _ _)).
+    rewrite <- (fsim_embed (map_normalize2 _ _ _)).
+    rewrite <- (st_cc_map_id ccA).
+    eapply st_map_monotonicity_cc.
+    rewrite (fsim_embed (normalize_comp_fsim_sk1 _ _ sk)).
+    rewrite <- (fsim_embed (normalize_comp_fsim_sk2 _ _ sk)).
+    assert (H1: ST.forward_simulation
+                &1 &1 (comp_semantics' (normalize_sem (L1s @ pstate L2s)) (normalize_sem L2s) sk)
+                      (comp_semantics' (normalize_sem L1s @ pstate L2s) (normalize_sem L2s) sk)).
+    {
+      eapply st_fsim_lcomp_sk.
+      instantiate (1 := &1).
+      apply fsim_embed. apply fsim_lift_normalize1.
+      reflexivity. all: easy.
+    }
+    rewrite H1. clear H1.
+    assert (H2: ST.forward_simulation
+                &1 &1 (comp_semantics' (normalize_sem L1t @ pstate L2t) (normalize_sem L2t) sk)
+                      (comp_semantics' (normalize_sem (L1t @ pstate L2t)) (normalize_sem L2t) sk)).
+    {
+      assert (skel L2t = skel L2s). destruct HL2. destruct X0. easy.
+      assert (skel L1t = skel L1s). destruct HL1. destruct X0. easy.
+      eapply st_fsim_lcomp_sk.
+      instantiate (1 := &1).
+      apply fsim_embed. apply fsim_lift_normalize2.
+      reflexivity.
+      cbn. rewrite H0. easy.
+      cbn. rewrite H. easy.
+    }
+    rewrite <- H2. apply X.
+  Qed.
+
+End COMP.
+
+(** A simplified condition for ccB ⊑ ccA, where the wB is a substructure of
+    wA. Additional invariant is required on wA to constrain the redundant
+    information *)
+Section CCREF.
+
+  Context {li1 li2} (ccA ccB: ST.callconv li1 li2).
+
+  Variable F: ST.ccworld ccA -> ST.ccworld ccB.
+  Variable I: ST.ccworld ccA -> Prop.
+  Hypothesis F_init: F (@pset_init (ST.ccworld ccA) _) = @pset_init (ST.ccworld ccB) _.
+  Hypothesis I_init: I (@pset_init (ST.ccworld ccA) _).
+  Hypothesis I_ext_step: forall wa wa1, I wa -> wa :-> wa1 -> I wa1.
+  Hypothesis F_int_step: forall wa1 wa2, wa1 *-> wa2 -> F wa1 *-> F wa2.
+  Hypothesis F_ext_step:
+    forall wa wb1, F wa :-> wb1 -> exists wa1, wa :-> wa1 /\ F wa1 = wb1.
+  Hypothesis F_mq:
+    forall wa q1 q2, I wa -> ST.match_query ccB (F wa) q1 q2 -> ST.match_query ccA wa q1 q2.
+  Hypothesis F_mr:
+    forall wa r1 r2, ST.match_reply ccA wa r1 r2 -> ST.match_reply ccB (F wa) r1 r2 /\ I wa.
+
+  Inductive sub_inv: ST.ccworld ccA -> ST.ccworld ccB -> Prop :=
+  | sub_inv_intro wa wb: I wa -> F wa :-> wb -> sub_inv wa wb.
+  Inductive sub_ms: ST.ccworld ccA -> ST.ccworld ccB -> @state li1 li1 1 -> @state li2 li2 1 -> Prop :=
+  | sub_ms_q q1 q2 wa wb:
+    I wa -> F wa = wb -> ST.match_query ccB wb q1 q2 ->
+    sub_ms wa wb (st_q q1) (st_q q2)
+  | sub_ms_r r1 r2 wa wb:
+    I wa -> F wa = wb -> ST.match_reply ccB wb r1 r2 ->
+    sub_ms wa wb (st_r r1) (st_r r2).
+
+  Lemma st_ccref_sub: st_ccref ccB ccA.
+  Proof.
+    apply st_normalize_fsim. constructor.
+    eapply ST.Forward_simulation with
+      (ltof _ (fun (_: unit) => 0)) (fun _ wa wb _ => sub_ms wa wb)
+      (fun wa wb => sub_inv wa wb); try easy.
+    - intros. inv H. constructor; eauto. etransitivity; eauto.
+    - constructor; eauto. rewrite F_init. reflexivity.
+    - intros wa wb se HI. inv HI.
+      constructor.
+      + intros q1 q2 s1 wb1 Hb Hq Hx. exists tt. inv Hx. exists (st_q q2).
+        split. constructor.
+        edestruct F_ext_step as (wa1 & Ha1 & Ha2).
+        etransitivity; eauto. subst.
+        exists wa1, (F wa1). repeat split; try easy.
+        constructor; eauto.
+      + intros wa1 wb1 [] s1 s2 r1 Hs Hx. inv Hx.
+        inv Hs. exists r2. split. constructor.
+        exists (F wa1). repeat split; easy.
+      + intros wa1 wb1 [] s1 s2 q1 Hs Hx. inv Hx. inv Hs.
+        exists q2. split. constructor.
+        exists wa1. split. reflexivity. split. apply F_mq; auto.
+        intros r1 r2 s1' wa2 Ha2 Hr Hy.
+        inv Hy. eexists tt, _. split. constructor.
+        eexists wa2, (F wa2). repeat split; eauto. easy.
+        constructor; eapply F_mr in Hr; easy.
+      + intros. easy.
+  Qed.
+
+End CCREF.
+
+Lemma lift_comp_ccref `{PSet S1} `{PSet S2} `{PSet S3}
+      `(cc1: ST.callconv liA liB) `(cc2: ST.callconv liB liC):
+  st_ccref (ST.callconv_lift (ST.cc_compose cc1 cc2) S1 S3)
+           (ST.cc_compose (ST.callconv_lift cc1 S1 S2) (ST.callconv_lift cc2 S2 S3)).
+Proof.
+  match goal with
+  | |- st_ccref ?x ?y => set (w1 := ST.ccworld x); set (w2 := ST.ccworld y)
+  end.
+  cbn in *.
+  set (F := fun '((w1, s1, _, (w2, _, s3)):w2) => (w1, w2, s1, s3)).
+  set (I := fun '((_, _, s2, (_, s2', _)):w2) => s2 = s2').
+  eapply st_ccref_sub with F I; intros; cbn in *; eprod_crush; subst; try easy.
+  - cbn in *. eprod_crush. subst. eexists (_, _, _, (_, _, _)). cbn.
+    repeat split; eauto.
+  - cbn in *. eprod_crush. subst.
+    eexists (_, _). repeat split; eauto.
+  - cbn in *. eprod_crush. subst.
+    repeat split; eauto.
+Qed.
+
+Section ENCAP_COMP_FSIM.
+
+  Context `(ccA1: ST.callconv liAs liAn) `(ccA2: ST.callconv liAn liAf)
+          `(ccB1: ST.callconv liBs liBn) `(ccB2: ST.callconv liBn liBf)
+          (Ls: liAs +-> liBs) (Ln: liAn +-> liBn) (Lf: liAf +-> liBf).
+  Context (H1: E.forward_simulation ccA1 ccB1 Ls Ln)
+          (H2: E.forward_simulation ccA2 ccB2 Ln Lf).
+
+  (** Lemma 3.11 *)
+  Lemma encap_fsim_vcomp:
+    E.forward_simulation (ST.cc_compose ccA1 ccA2)
+                         (ST.cc_compose ccB1 ccB2) Ls Lf.
+  Proof.
+    unfold E.forward_simulation in *.
+    exploit @st_fsim_vcomp. exact H1. exact H2. clear.
+    intros X.
+    rewrite @lift_comp_ccref. apply X.
+  Qed.
+End ENCAP_COMP_FSIM.
+
+Lemma cc_lift_unit `(cc: ST.callconv liA liB):
+  st_ccref (ST.callconv_lift cc unit unit)
+           (st_callconv_map (li_iso_inv _) (li_iso_inv _) cc).
+Proof.
+  match goal with
+  | |- st_ccref ?x ?y => set (w1 := ST.ccworld x); set (w2 := ST.ccworld y)
+  end.
+  cbn in *.
+  set (F := fun '((w, _, _):w1) => w).
+  set (G := fun (w:w2) => (w, tt, tt)).
+  eapply st_ccref_intro with G F;
+    intros; cbn in *; eprod_crush; cbn; try easy.
+Qed.
+
+Lemma fsim_normalize `(ccA: callconv liA1 liA2) `(ccB: callconv liB1 liB2) L1 L2:
+  forward_simulation ccA ccB L1 L2 ->
+  CAT.forward_simulation ccA ccB L1 L2.
+Proof.
+  intros HL. assert (Hsk: skel L1 = skel L2).
+  destruct HL. apply (fsim_skel X).
+  unfold CAT.forward_simulation, normalize_sem, left_comp_id, right_comp_id.
+  rewrite Hsk.
+  eapply categorical_compose_simulation'.
+  apply ccref_to_fsim. reflexivity.
+  eapply categorical_compose_simulation'.
+  apply HL. apply ccref_to_fsim. reflexivity.
+  rewrite Hsk.  all: cbn; (apply Linking.linkorder_refl || apply CategoricalComp.id_skel_order).
+Qed.
+
+Lemma encap_fsim_embed `(ccA: callconv liA1 liA2) `(ccB: callconv liB1 liB2)
+      `{World (ccworld ccA)} `{World (ccworld ccB)} L1 L2:
+  forward_simulation ccA ccB L1 L2 ->
+  E.forward_simulation &ccA &ccB
+                       (semantics_embed L1) (semantics_embed L2).
+Proof.
+  intros. unfold E.forward_simulation, semantics_embed. cbn.
+  rewrite cc_lift_unit. rewrite <- (st_cc_map_id &ccA).
+  unfold STCAT.forward_simulation.
+  rewrite (fsim_embed (map_normalize1 _ (li_iso_inv li_iso_unit) _)).
+  rewrite <- (fsim_embed (map_normalize2 _ (li_iso_inv li_iso_unit) _)).
+  apply st_map_monotonicity_cc.
+  apply fsim_embed. apply fsim_normalize. assumption.
+Qed.
+
+(** ** Simulation Convention FBK *)
+Definition callconv_fbk `{PSet K1} `{PSet K2}
+        `(cc: ST.callconv (li1@K1) (li2@K2)): ST.callconv li1 li2 :=
+  {|
+    ST.ccworld := ST.ccworld cc * K1 * K2;
+    ST.match_query '(w, k1, k2) q1 q2 := ST.match_query cc w (q1, k1) (q2, k2);
+    ST.match_reply '(w, k1, k2) r1 r2 := ST.match_reply cc w (r1, k1) (r2, k2);
+  |}.
+
+Lemma ccref_lift `{PSet K1} `{PSet K2} {li1 li2} (ccA ccB: ST.callconv li1 li2):
+  st_ccref ccA ccB -> st_ccref (ST.callconv_lift ccA K1 K2) (ST.callconv_lift ccB K1 K2).
+Proof.
+  unfold st_ccref. intros A. unfold STCAT.forward_simulation.
+  assert (X: forward_simulation 1 1 (@normalize_sem (li1@K1) _ 1) (normalize_sem 1 @ K1)).
+  {
+    etransitivity. 2: apply lift_categorical_comp2.
+    eapply categorical_compose_simulation'. apply lift_unit1.
+    etransitivity. 2: apply lift_categorical_comp2.
+    eapply categorical_compose_simulation'. 1-2: apply lift_unit1.
+    all: apply Linking.linkorder_refl.
+  }
+  assert (Y: forward_simulation 1 1 (@normalize_sem li2 _ 1 @ K2) (normalize_sem 1)).
+  {
+    etransitivity. apply lift_categorical_comp1.
+    eapply categorical_compose_simulation'. apply lift_unit2.
+    etransitivity. apply lift_categorical_comp1.
+    eapply categorical_compose_simulation'. 1-2: apply lift_unit2.
+    all: apply Linking.linkorder_refl.
+  }
+  rewrite (fsim_embed X). rewrite <- (fsim_embed Y).
+  apply st_fsim_lift. apply A.
+Qed.
+
+(** ** FBK vs LIFT *)
+
+(** A simplified condition for ccB ⊑ ccA, where wA is a substructure of wB *)
+Section CCREF.
+
+  Context {li1 li2} (ccA ccB: ST.callconv li1 li2).
+
+  Variable F: ST.ccworld ccB -> ST.ccworld ccA.
+  Variable I: ST.ccworld ccB -> Prop.
+  Hypothesis F_init: F (@pset_init (ST.ccworld ccB) _) = @pset_init (ST.ccworld ccA) _.
+  Hypothesis F_ext_step: forall x y, x :-> y -> F x :-> F y.
+  Hypothesis F_int_step:
+    forall wb1 wa2, F wb1 *-> wa2 -> exists wb2, wa2 = F wb2 /\ wb1 *-> wb2 /\ (I wb1 -> I wb2).
+  Hypothesis F_mq:
+    forall wb q1 q2, ST.match_query ccB wb q1 q2 -> ST.match_query ccA (F wb) q1 q2 /\ I wb.
+  Hypothesis F_mr:
+    forall wb r1 r2, I wb -> ST.match_reply ccA (F wb) r1 r2 -> ST.match_reply ccB wb r1 r2.
+
+  Inductive super_inv: ST.ccworld ccA -> ST.ccworld ccB -> Prop :=
+  | super_inv_intro wa wb: wa :-> F wb -> super_inv wa wb.
+  Inductive super_ms: ST.ccworld ccA -> ST.ccworld ccB -> @state li1 li1 1 -> @state li2 li2 1 -> Prop :=
+  | super_ms_q q1 q2 wa wb:
+    I wb -> wa = F wb -> ST.match_query ccB wb q1 q2 ->
+    super_ms wa wb (st_q q1) (st_q q2)
+  | super_ms_r r1 r2 wa wb:
+    I wb -> wa = F wb -> ST.match_reply ccB wb r1 r2 ->
+    super_ms wa wb (st_r r1) (st_r r2).
+
+  Lemma st_ccref_super: st_ccref ccB ccA.
+  Proof.
+    apply st_normalize_fsim. constructor.
+    eapply ST.Forward_simulation with
+      (ltof _ (fun (_: unit) => 0)) (fun _ wa wb _ => super_ms wa wb)
+      (fun wa wb => super_inv wa wb); try easy.
+    - intros. inv H. constructor. etransitivity; eauto.
+    - constructor. rewrite F_init. reflexivity.
+    - intros wa wb se Hi. inv Hi.
+      constructor.
+      + intros q1 q2 s1 wb1 Hb Hq Hx. exists tt. inv Hx. exists (st_q q2).
+        split. constructor.
+        exists (F wb1), wb1. repeat split; try easy.
+        * etransitivity; eauto.
+        * constructor; eauto. apply F_mq in Hq. apply Hq.
+      + intros wa1 wb1 [] s1 s2 r1 Hs Hx. inv Hx.
+        inv Hs. exists r2. split. constructor.
+        exists wb1. repeat split; easy.
+      + intros wa1 wb1 [] s1 s2 q1 Hs Hx. inv Hx. inv Hs.
+        exists q2. split. constructor.
+        exists (F wb1). split. reflexivity. split. apply F_mq; auto.
+        intros r1 r2 s1' wa2 Ha2 Hr Hy.
+        inv Hy. eexists tt, _. split. constructor.
+        destruct (F_int_step _ _ Ha2) as (wb2 & Hb1 & Hb2 & Hb3).
+        eexists wa2, wb2. repeat split; try easy.
+        constructor; eauto.
+        apply F_mr; subst; eauto.
+      + intros. easy.
+  Qed.
+
+End CCREF.
+
+Lemma cc_fbk_lift1 `{PSet K1} `{PSet K2} `(cc: ST.callconv li1 li2):
+  st_ccref (callconv_fbk (ST.callconv_lift cc K1 K2)) cc.
+Proof.
+  match goal with
+  | |- st_ccref ?x ?y => set (w1 := ST.ccworld x); set (w2 := ST.ccworld y)
+  end.
+  cbn in *.
+  set (F := fun '((w, _, _, _, _):w1) => w).
+  set (I := fun '((_, k1, k2, k1', k2'):w1) => k1 = k1' /\ k2 = k2').
+  eapply st_ccref_super with F I;
+    intros; cbn in *; eprod_crush; subst; try easy.
+  eexists (_, _, _, _, _). repeat split. eauto.
+  Unshelve. all: eauto.
+Qed.
+
+Lemma cc_fbk_lift2 `{PSet K1} `{PSet K2} `(cc: ST.callconv li1 li2):
+  st_ccref cc (callconv_fbk (ST.callconv_lift cc K1 K2)).
+Proof.
+  match goal with
+  | |- st_ccref ?x ?y => set (w1 := ST.ccworld x); set (w2 := ST.ccworld y)
+  end.
+  cbn in *.
+  set (F := fun '((w, _, _, _, _):w2) => w).
+  set (I := fun '((_, k1, k2, k1', k2'):w2) => k1 = k1' /\ k2 = k2').
+  eapply st_ccref_sub with F I;
+    intros; cbn in *; eprod_crush; subst; try easy.
+  eexists (_, _, _, _, _). repeat split. easy.
+Qed.
+
+(** A simplified condition for ccB ⊑ ccA, where wA is a substructure of wB *)
+Section CCREF.
+
+  Context {li1 li2} (ccA ccB: ST.callconv li1 li2).
+
+  Variable F: ST.ccworld ccB -> ST.ccworld ccA.
+  Variable I: ST.ccworld ccB -> Prop.
+  Hypothesis F_init: @pset_init (ST.ccworld ccA) _ :-> F (@pset_init (ST.ccworld ccB) _).
+  (* F (pset_init (ST.ccworld ccB)) = pset_init (ST.ccworld ccA). *)
+  Hypothesis I_init: I (@pset_init (ST.ccworld ccB) _).
+  Hypothesis I_ext_step: forall wb wb1, I wb -> wb :-> wb1 -> I wb1.
+  Hypothesis F_ext_step: forall x y, x :-> y -> F x :-> F y.
+  Hypothesis F_int_step:
+    forall wb1 wa2, F wb1 *-> wa2 ->
+               forall r1 r2, exists wb2, wa2 = F wb2 /\ wb1 *-> wb2
+                               /\ (I wb1 -> I wb2)
+                               /\ (ST.match_reply ccA wa2 r1 r2 ->
+                                  ST.match_reply ccB wb2 r1 r2).
+  Hypothesis F_mq:
+    forall wb q1 q2, I wb -> ST.match_query ccB wb q1 q2 -> ST.match_query ccA (F wb) q1 q2.
+
+  Inductive fbk1_inv: ST.ccworld ccA -> ST.ccworld ccB -> Prop :=
+  | fbk1_inv_intro wa wb: I wb -> wa :-> F wb -> fbk1_inv wa wb.
+  Inductive fbk1_ms: ST.ccworld ccA -> ST.ccworld ccB -> @state li1 li1 1 -> @state li2 li2 1 -> Prop :=
+  | fbk1_ms_q q1 q2 wa wb:
+    I wb -> wa = F wb -> ST.match_query ccB wb q1 q2 ->
+    fbk1_ms wa wb (st_q q1) (st_q q2)
+  | fbk1_ms_r r1 r2 wa wb:
+    I wb -> wa = F wb -> ST.match_reply ccB wb r1 r2 ->
+    fbk1_ms wa wb (st_r r1) (st_r r2).
+
+  Lemma st_ccref_fbk1: st_ccref ccB ccA.
+  Proof.
+    apply st_normalize_fsim. constructor.
+    eapply ST.Forward_simulation with
+      (ltof _ (fun (_: unit) => 0)) (fun _ wa wb _ => fbk1_ms wa wb)
+      (fun wa wb => fbk1_inv wa wb); try easy.
+    - intros. inv H. constructor; eauto. etransitivity; eauto.
+    - intros wa wb se Hi. inv Hi.
+      constructor.
+      + intros q1 q2 s1 wb1 Hb Hq Hx. exists tt. inv Hx. exists (st_q q2).
+        split. constructor.
+        exists (F wb1), wb1. repeat split; try easy.
+        * etransitivity; eauto.
+        * constructor; eauto.
+      + intros wa1 wb1 [] s1 s2 r1 Hs Hx. inv Hx.
+        inv Hs. exists r2. split. constructor.
+        exists wb1. repeat split; easy.
+      + intros wa1 wb1 [] s1 s2 q1 Hs Hx. inv Hx. inv Hs.
+        exists q2. split. constructor.
+        exists (F wb1). split. reflexivity. split. apply F_mq; auto.
+        intros r1 r2 s1' wa2 Ha2 Hr Hy.
+        inv Hy. eexists tt, _. split. constructor.
+        destruct (F_int_step _ _ Ha2 r1 r2) as (wb2 & Hb1 & Hb2 & Hb3 & HR).
+        eexists wa2, wb2. repeat split; try easy.
+        constructor; eauto.
+      + intros. easy.
+  Qed.
+
+End CCREF.
+
+Lemma cc_lift_fbk1 `{PSet K1} `{PSet K2} `(cc: ST.callconv (li1@K1) (li2@K2)):
+  st_ccref (ST.callconv_lift (callconv_fbk cc) K1 K2) cc.
+Proof.
+  match goal with
+  | |- st_ccref ?x ?y => set (w1 := ST.ccworld x); set (w2 := ST.ccworld y)
+  end.
+  cbn in *.
+  set (F := fun '((w, _, _, _, _):w1) => w).
+  set (I := fun '((_, k1, k2, k1', k2'):w1) => k1 = k1' /\ k2 = k2').
+  eapply st_ccref_fbk1 with F I;
+    intros; cbn in *; eprod_crush; subst; try easy.
+  eexists (_, _, _, _, _). repeat split. eauto.
+  intros; cbn in *. eprod_crush. repeat split; eauto.
+  cbn in *. eprod_crush. subst; eauto.
+Qed.
+
+Lemma cc_lift_fbk2 `{PSet K1} `{PSet K2} `(cc: ST.callconv (li1@K1) (li2@K2)):
+  st_ccref cc (ST.callconv_lift (callconv_fbk cc) K1 K2).
+Proof.
+  match goal with
+  | |- st_ccref ?x ?y => set (w1 := ST.ccworld x); set (w2 := ST.ccworld y)
+  end.
+  cbn in *.
+  set (F := fun '((w, _, _, _, _):w2) => w).
+  set (I := fun '((_, k1, k2, k1', k2'):w2) => k1 = k1' /\ k2 = k2').
+  eapply st_ccref_sub with F I;
+    intros; cbn in *; eprod_crush; subst; try easy.
+  eexists (_, _, _, _, _). repeat split. easy.
+  cbn in *. admit.
+  cbn in *.
+Abort.
+
+Lemma encap_fsim_fbk `{PSet K1} `{PSet K2}
+      `(ccA: ST.callconv liA1 liA2) `(ccB: ST.callconv (liB1@K1) (liB2@K2)) L1 L2:
+  E.forward_simulation ccA ccB L1 L2 ->
+  E.forward_simulation ccA (callconv_fbk ccB) (semantics_fbk L1) (semantics_fbk L2).
+Proof.
+  unfold E.forward_simulation. cbn. intros HL.
+  rewrite cc_lift_twice.
+  unfold STCAT.forward_simulation.
+  rewrite (fsim_embed (map_normalize1 _ _ _)).
+  rewrite <- (fsim_embed (map_normalize2 _ _ _)).
+  rewrite <- (st_cc_map_id ccA).
+  eapply st_map_monotonicity_cc.
+  pose proof (@ccref_lift (pstate L1) _ (pstate L2) _  _ _ _ _ (cc_lift_fbk1 ccB)) as Hcc.
+  assert (X: STCAT.forward_simulation ccA (ST.callconv_lift (ST.callconv_lift (callconv_fbk ccB) K1 K2) (pstate L1) (pstate L2)) L1 L2).
+  {
+    rewrite Hcc. apply HL.
+  }
+  apply X.
+Qed.
+
+(** ** REVEAL Simulation Convention *)
+
+Program Definition cc_reveal `{PSet K} {li} : ST.callconv li (li@K) :=
+  {|
+    ST.ccworld := K;
+    ST.match_query k q1 '(q2, kq) := q1 = q2 /\ k = kq;
+    ST.match_reply k r1 '(r2, kr) := r1 = r2 /\ k = kr;
+  |}.
+
+Lemma cc_lift_reveal {li} `{PSet K1} `{PSet K2}:
+  st_ccref
+    (ST.callconv_lift (cc_reveal (li:=li)) (K2 * K1) K1)
+    (st_callconv_map li_iso_assoc li_iso_id &1).
+Proof.
+  match goal with
+  | |- st_ccref ?x ?y => set (w1 := ST.ccworld x); set (w2 := ST.ccworld y)
+  end.
+  cbn in *.
+  set (F := fun _:w1 => tt).
+  set (I := fun '((k2, (kk2, k1), kk1):w1) => k1 = kk1 /\ k2 = kk2).
+  eapply st_ccref_fbk1 with F I.
+  all: intros; cbn in *; eprod_crush; subst; try easy.
+  - eexists (_, (_, _), _). cbn in *. repeat split.
+    eprod_crush. inv H2. easy.
+    eprod_crush. inv H2. easy.
+  - inv H1. reflexivity.
+Qed.
+
+Section REVEAL.
+
+  Lemma sem_map_id `(L: semantics liA liB):
+    L = semantics_map L lf lf.
+  Proof.
+    unfold semantics_map. destruct L. cbn. f_equal.
+    extensionality se.
+    unfold lts_map. destruct (activate se).
+    cbn. f_equal.
+    - extensionality x. extensionality y. extensionality z.
+      apply propositional_extensionality. split.
+      + intros. eexists; split; eauto. reflexivity.
+      + intros. eprod_crush. subst. apply H0.
+    - extensionality x. extensionality y.
+      apply propositional_extensionality. split.
+      + intros. eexists; split; eauto. reflexivity.
+      + intros. eprod_crush. subst. apply H0.
+  Qed.
+
+  Lemma fsim_reveal `{PSet K} {liA liB} (L: liA +-> liB@K):
+    E.forward_simulation &1 cc_reveal (semantics_fbk L) L.
+  Proof.
+    unfold E.forward_simulation. cbn. rewrite cc_lift_reveal.
+    unfold STCAT.forward_simulation.
+    rewrite (fsim_embed (map_normalize1 _ _ _)).
+    rewrite <- (st_cc_map_id &1).
+    rewrite (sem_map_id (normalize_sem L)) at 2.
+    eapply st_map_monotonicity_cc.
+    reflexivity.
+  Qed.
+
+End REVEAL.
